ReOrg Walk file

Kura/Walk/Operation.lean
@@ -1,64 +1,12 @@
-import Kura.Operation.Subgraph
-import Kura.Operation.Minor
-import Mathlib.Data.Finset.Lattice.Basic
-import Kura.Dep.List
-import Mathlib.Data.Nat.PartENat
+import Kura.Walk.Defs
 
-open Set Function List Nat
-variable {α β : Type*} {G H : Graph α β} {u v x y z : α} {e e' f g : β} {S T U: Set α}
-  {F F' : Set β}
+
 namespace Graph
-
-
-inductive Walk (α β : Type*) where
-| nil (u : α) : Walk α β
-| cons (u : α) (e : β) (W : Walk α β) : Walk α β
-
-variable {w w₁ w₂ : Walk α β}
+open Set Function List Nat Walk
+variable {α β : Type*} {G H : Graph α β} {u v x y z : α} {e e' f g : β} {S T U: Set α}
+  {F F' : Set β} {w w₁ w₂ : Walk α β}
 namespace Walk
 
-def Nonempty : Walk α β → Prop
-| nil _ => False
-| cons _ _ _ => True
-
-def first : Walk α β → α
-| nil x => x
-| cons x _ _ => x
-
-def last : Walk α β → α
-| nil x => x
-| cons _ _ w => w.last
-
-def ValidIn (w : Walk α β) (G : Graph α β) : Prop :=
-  match w with
-  | nil x => x ∈ G.V
-  | cons x e w => G.Inc₂ e x w.first ∧ w.ValidIn G
-
-def vx : Walk α β → List α
-| nil x => [x]
-| cons x _e w => x :: w.vx
-
-instance : Membership α (Walk α β) where
-  mem w x := x ∈ w.vx
-
-instance [DecidableEq α] : Decidable (x ∈ w) := by
-  change Decidable (x ∈ w.vx)
-  infer_instance
-
-@[simp]
-lemma mem_notation : (x ∈ w.vx) = (x ∈ w) := rfl
-
-def vxSet : Walk α β → Set α := fun w => {x | x ∈ w}
-
-def edge : Walk α β → List β
-| nil _ => []
-| cons _ e w => e :: w.edge
-
-def edgeSet : Walk α β → Set β := fun w => {e | e ∈ w.edge}
-
-def length : Walk α β → ℕ
-| nil _ => 0
-| cons _ _ w => w.length + 1
 
 def concat : Walk α β → β → α → Walk α β
 | nil x, e, y => cons x e (nil y)
@@ -77,10 +25,10 @@ instance instAppend : Append (Walk α β) where
   append := append
 
 def IsPrefix : Walk α β → Walk α β → Prop :=
-  fun W w => ∃ w', W = w ++ w'
+  fun W w => ∃ w', W = w ++ w' ∧ w.last = w'.first
 
 def IsSuffix : Walk α β → Walk α β → Prop :=
-  fun W w => ∃ w', W = w' ++ w
+  fun W w => ∃ w', W = w' ++ w ∧ w'.last = w.first
 
 def reverse : Walk α β → Walk α β
 | nil x => nil x
@@ -93,9 +41,6 @@ def firstAt [DecidableEq α] (w : Walk α β) (u : α) (h : u ∈ w) : Walk α �
     if hin : u ∈ w
     then firstAt w u hin
     else cons x e w
-
-@[simp]
-lemma cons_length : (cons x e w).length = w.length + 1 := rfl
 
 lemma firstAt_length_le [DecidableEq α] {w : Walk α β} (h : u ∈ w) : (firstAt w u h).length ≤ w.length := by
   match w with
@@ -117,8 +62,6 @@ def dedup [DecidableEq α] : Walk α β → Walk α β
   else cons x e (dedup w)
 termination_by w => w.length
 
-@[simp] lemma cons_vx : (cons x e w).vx = x :: w.vx := rfl
-
 def endIf {P : α → Prop} [DecidablePred P] (w : Walk α β) (h : ∃ u ∈ w, P u) : Walk α β :=
   match w with
   | nil x => nil x
@@ -127,177 +70,230 @@ def endIf {P : α → Prop} [DecidablePred P] (w : Walk α β) (h : ∃ u ∈ w,
     then nil x
     else cons x e (endIf w (by simpa [← mem_notation, hP] using h))
 
-end Walk
 
-@[mk_iff]
-structure IsWalkFrom (G : Graph α β) (S T : Set α) (W : Walk α β) : Prop where
-  validIn : W.ValidIn G
-  first_mem : W.first ∈ S
-  last_mem : W.last ∈ T
-
-namespace Walk
-
-@[simp] lemma nil_vx : (nil x : Walk α β).vx = [x] := rfl
-
-@[simp] lemma nil_edge : (nil x : Walk α β).edge = [] := rfl
-
-@[simp] lemma nil_length : (nil x : Walk α β).length = 0 := rfl
-
-@[simp] lemma nil_first : (nil x : Walk α β).first = x := rfl
-
-@[simp] lemma nil_last : (nil x : Walk α β).last = x := rfl
-
-@[simp] lemma nil_validIn_iff : (nil x : Walk α β).ValidIn G ↔ x ∈ G.V := by
-  simp only [ValidIn]
-
-@[simp] lemma nil_injective : Injective (nil : α → Walk α β) := by
-  rintro x y h
-  rwa [nil.injEq] at h
-
--- @[simp] lemma nil_inj : (nil x : Walk α β) = nil y ↔ x = y := by
---   rw [nil.injEq]
-
-@[simp] lemma cons_edge : (cons x e w).edge = e :: w.edge := rfl
-
-@[simp] lemma cons_first : (cons x e w).first = x := rfl
-
-@[simp] lemma cons_last : (cons x e w).last = w.last := rfl
-
-@[simp] lemma cons_validIn (hw : w.ValidIn G) (he : G.Inc₂ e x w.first) :
-  (cons x e w).ValidIn G := ⟨he, hw⟩
-
-@[simp] lemma cons_validIn_iff : (cons x e w).ValidIn G ↔ G.Inc₂ e x w.first ∧ w.ValidIn G :=
-  ⟨id, id⟩
-
-lemma ValidIn.of_cons (hw : (cons x e w).ValidIn G) : w.ValidIn G := by
-  rw [cons_validIn_iff] at hw
-  exact hw.2
-
-lemma cons_vx_nodup (h : (cons x e w).vx.Nodup) : w.vx.Nodup := by
-  simp only [cons_vx, nodup_cons] at h
-  exact h.2
-
-lemma vx_ne_nil : w.vx ≠ [] := by
-  match w with
-  | nil x => simp
-  | cons x e w => simp
+/-- Properties of dropLast operation -/
+@[simp]
+lemma dropLast_nil : (nil x : Walk α β).dropLast = nil x := rfl
 
 @[simp]
-lemma mem_vx_nil_iff : x ∈ (nil u : Walk α β) ↔ x = u := by simp [← mem_notation]
+lemma dropLast_cons_nil : (cons x e (nil y) : Walk α β).dropLast = nil x := rfl
 
 @[simp]
-lemma mem_vx_cons_iff : x ∈ (cons u e w) ↔ x = u ∨ x ∈ w := by simp [← mem_notation]
+lemma dropLast_cons_cons :
+  (cons x e (cons y e' w) : Walk α β).dropLast = cons x e ((cons y e' w).dropLast) := rfl
 
 @[simp]
-lemma mem_edge_nil_iff : e ∈ (nil u : Walk α β).edge ↔ False := by simp
+lemma dropLast_first {w : Walk α β} (h : w.Nonempty) : (w.dropLast).first = w.first := by
+  match w with
+  | .nil x => simp at h
+  | .cons x e (.nil y) => simp
+  | .cons x e (cons y e' w) => simp
 
 @[simp]
-lemma mem_edge_cons_iff : e ∈ (cons u e' w).edge ↔ e = e' ∨ e ∈ w.edge := by simp
+lemma dropLast_vx {w : Walk α β} (h : w.Nonempty) : (w.dropLast).vx = w.vx.dropLast := by
+  match w with
+  | .nil x => simp only [Nonempty.not_nil] at h
+  | .cons x e (.nil y) => simp only [dropLast, nil_vx, cons_vx, dropLast_cons₂, dropLast_single]
+  | .cons x e (cons y e' w) =>
+    simp only [dropLast, cons_vx, dropLast_cons₂, List.cons.injEq, true_and]
+    rw [← cons_vx (e := e')]
+    apply dropLast_vx (by simp)
 
 @[simp]
-lemma first_vx_mem : w.first ∈ w := by
+lemma dropLast_edge {w : Walk α β} (h : w.Nonempty) : (w.dropLast).edge = w.edge.dropLast := by
   match w with
-  | nil x => simp
-  | cons x e w => simp
+  | .nil x => simp only [Nonempty.not_nil] at h
+  | .cons x e (.nil y) => simp only [dropLast, nil_edge, cons_edge, dropLast_single]
+  | .cons x e (cons y e' w) =>
+    simp only [dropLast, cons_edge, dropLast_cons₂, List.cons.injEq, true_and]
+    exact dropLast_edge (by simp)
 
-lemma first_eq_vx_head {w : Walk α β} : w.first = w.vx.head vx_ne_nil := by
+lemma dropLast_validIn {w : Walk α β} (hVd : w.ValidIn G) : (w.dropLast).ValidIn G := by
   match w with
-  | nil x => rfl
-  | cons x e w => rfl
+  | .nil x => simp only [dropLast, hVd]
+  | .cons x e (.nil y) =>
+    simp only [cons_validIn, nil_first, nil_validIn] at hVd
+    exact hVd.1.vx_mem_left
+  | .cons x e (cons y e' w) =>
+    rw [dropLast, cons_validIn, dropLast_first (by simp)]
+    rw [cons_validIn] at hVd
+    exact ⟨hVd.1, dropLast_validIn hVd.2⟩
+
+lemma mem_dropLast_or_last_of_mem {w : Walk α β} (hu : u ∈ w) : u ∈ w.dropLast ∨ u = w.last := by
+  match w with
+  | .nil x => simpa using hu
+  | .cons x e (.nil y) =>
+    simp only [mem_cons_iff, mem_nil_iff] at hu
+    obtain rfl | rfl := hu <;> simp
+  | .cons x e (cons y e' w) =>
+    simp only [mem_cons_iff] at hu
+    obtain rfl | rfl | hu := hu
+    · simp
+    · simp only [dropLast_cons_cons, mem_cons_iff, cons_last]
+      have := mem_dropLast_or_last_of_mem (by simp : u ∈ (cons u e' w))
+      rw [cons_last] at this
+      tauto
+    · simp only [dropLast_cons_cons, mem_cons_iff, cons_last]
+      have := mem_dropLast_or_last_of_mem (by simp [hu] : u ∈ (cons y e' w))
+      rw [cons_last] at this
+      tauto
+
+lemma mem_of_mem_dropLast {w : Walk α β} (h : u ∈ w.dropLast) : u ∈ w := by
+  match w with
+  | .nil x => simpa using h
+  | .cons x e (.nil y) => simp_all only [dropLast_cons_nil, mem_nil_iff, mem_cons_iff, true_or]
+  | .cons x e (cons y e' w) =>
+    simp only [dropLast_cons_cons, mem_cons_iff] at h ⊢
+    obtain rfl | h := h
+    · left
+      rfl
+    · have := mem_of_mem_dropLast (w := cons y e' w) (by simpa only [Nonempty.cons_true,
+      dropLast_vx, cons_vx])
+      right
+      simpa only [mem_cons_iff] using this
+
+lemma mem_dropLast_or_last_of_mem_iff :
+    u ∈ w.dropLast ∨ u = w.last ↔ u ∈ w := by
+  refine ⟨?_, mem_dropLast_or_last_of_mem⟩
+  rintro (h | rfl)
+  · exact mem_of_mem_dropLast h
+  · exact last_mem
 
 @[simp]
-lemma last_vx_mem {w : Walk α β} : w.last ∈ w := by
+lemma dropLast_vxSet_of_isPath {w : Walk α β} (hP : G.IsPath w) (hn : w.Nonempty) :
+    (w.dropLast).vxSet = w.vxSet \ {w.last} := by
   match w with
-  | nil x => simp
-  | cons x e w =>
-    simp only [cons_vx, cons_last, mem_cons]
-    right
-    exact last_vx_mem
+  | .nil x => simp at hn
+  | .cons x e (.nil y) =>
+    simp only [dropLast_cons_nil, nil_vxSet, cons_vxSet, union_singleton, cons_last, nil_last,
+      mem_singleton_iff, insert_diff_of_mem]
+    rw [diff_singleton_eq_self]
+    simp only [mem_singleton_iff]
+    rintro rfl
+    simp at hP
+  | .cons x e (cons y e' w) =>
+    have := dropLast_vxSet_of_isPath (w := cons y e' w)
+    simp only [cons_isPath, Nonempty.cons_true, cons_vxSet, singleton_union, cons_last,
+      forall_const, and_imp, cons_first, mem_cons_iff, not_or, dropLast_cons_cons,
+      union_insert] at this hP ⊢
+    obtain ⟨⟨hP, h₂', hynin⟩, h₂, hne, hxnin⟩ := hP
+    rw [this hP h₂' hynin, ← insert_diff_of_not_mem, insert_comm]
+    simp only [mem_singleton_iff]
+    rintro rfl
+    simp only [last_mem, not_true_eq_false] at hxnin
 
-lemma last_eq_vx_getLast {w : Walk α β} : w.last = w.vx.getLast vx_ne_nil := by
-  match w with
-  | nil x => rfl
-  | cons x e w =>
-    simp only [cons_last, cons_vx, ne_eq, vx_ne_nil, not_false_eq_true, getLast_cons]
-    apply last_eq_vx_getLast
+@[simp]
+lemma last_not_mem_dropLast_of_isPath {w : Walk α β} (hP : G.IsPath w) (hn : w.Nonempty) :
+    w.last ∉ w.dropLast := by
+  rintro h
+  rw [← mem_vxSet_iff, dropLast_vxSet_of_isPath hP hn] at h
+  simp at h
 
-lemma ValidIn.mem_of_mem_vx {w : Walk α β} (h : w.ValidIn G) (hmem : x ∈ w) :
-    x ∈ G.V := by
-  match w with
-  | nil y =>
-    rw [mem_vx_nil_iff] at hmem
-    subst x
-    exact h
-  | cons y e w =>
-    obtain ⟨hbtw, hVd⟩ := h
-    obtain rfl | h : x = y ∨ x ∈ w := by simpa using hmem
-    · exact hbtw.vx_mem_left
-    · exact hVd.mem_of_mem_vx h
+/-- Properties of concat operation -/
+@[simp]
+lemma nil_concat : (nil x).concat e y = cons x e (nil y) := rfl
 
-lemma ValidIn.mem_of_mem_edge {w : Walk α β} (h : w.ValidIn G) (hmem : e ∈ w.edge) :
-    e ∈ G.E := by
-  match w with
-  | nil x => simp at hmem
-  | cons x e' w =>
-    obtain ⟨hbtw, hVd⟩ := h
-    obtain rfl | h : e = e' ∨ e ∈ w.edge := by simpa using hmem
-    · exact hbtw.edge_mem
-    · exact hVd.mem_of_mem_edge h
+@[simp]
+lemma cons_concat : (cons x e w).concat f y = cons x e (w.concat f y) := rfl
 
-lemma Nonempty.exists_cons : w.Nonempty → ∃ x e w', w = cons x e w' := by
+@[simp]
+lemma concat_first : (w.concat e v).first = w.first := by
   induction w with
-  | nil x => simp only [Nonempty, reduceCtorEq, exists_false, imp_self]
-  | cons x e w ih => simp only [cons.injEq, exists_and_left, exists_eq', and_true, implies_true]
-
-lemma Nonempty.iff_exists_cons : w.Nonempty ↔ ∃ x e w', w = cons x e w' := by
-  constructor
-  · apply Nonempty.exists_cons
-  · rintro ⟨x, e, w', rfl⟩
-    simp only [Nonempty, cons.injEq, exists_and_left, exists_eq', and_true, implies_true]
+  | nil x => simp [concat]
+  | cons x e w ih => simp [concat, ih]
 
 @[simp]
-lemma Nonempty.not_nil : ¬ (nil x : Walk α β).Nonempty := by
-  simp only [Nonempty, not_false_eq_true]
+lemma concat_last : (w.concat e v).last = v := by
+  induction w with
+  | nil x => simp [concat]
+  | cons x e w ih => simp [concat, ih]
 
 @[simp]
-lemma Nonempty.cons_true : (cons x e w).Nonempty := by
-  simp only [Nonempty]
+lemma concat_vx : (w.concat e v).vx = w.vx ++ [v] := by
+  induction w with
+  | nil x => simp [concat]
+  | cons x e w ih => simp [concat, ih]
 
 @[simp]
-lemma Nonempty.not_iff : ¬ w.Nonempty ↔ ∃ x, w = nil x := by
-  match w with
-  | nil x => simp only [not_nil, not_false_eq_true, nil.injEq, exists_eq']
-  | cons x e w => simp only [Nonempty, not_true_eq_false, reduceCtorEq, exists_false]
+lemma concat_edge : (w.concat e v).edge = w.edge ++ [e] := by
+  induction w with
+  | nil x => simp [concat]
+  | cons x e w ih => simp [concat, ih]
 
 @[simp]
-lemma Nonempty.iff_length_pos : 0 < w.length ↔ w.Nonempty := by
-  constructor
-  · rintro hlen
-    by_contra! h
-    simp only [not_iff] at h
-    obtain ⟨x, rfl⟩ := h
-    simp at hlen
-  · rw [Nonempty.iff_exists_cons]
-    rintro ⟨x, e, w, rfl⟩
-    simp only [cons_length, lt_add_iff_pos_left, add_pos_iff, lt_one_iff, pos_of_gt, or_true]
+lemma concat_length : (w.concat e v).length = w.length + 1 := by
+  induction w with
+  | nil x => simp [concat]
+  | cons x e w ih => simp [concat, ih]
 
-lemma first_eq_last_of_not_nonempty (h : ¬ w.Nonempty) : w.first = w.last := by
-  match w with
-  | nil x => simp only [nil_first, nil_last]
-  | cons x e w => simp only [Nonempty.cons_true, not_true_eq_false] at h
+lemma ValidIn.concat (hVd : w.ValidIn G) (h₂ : G.Inc₂ e w.last v) : (w.concat e v).ValidIn G := by
+  induction w with
+  | nil x =>
+    simp only [nil_validIn, nil_last] at hVd h₂
+    simp [concat, hVd, h₂, h₂.vx_mem_right]
+  | cons x e' w' ih =>
+    simp only [cons_validIn, cons_last, cons_concat, concat_first] at hVd h₂ ⊢
+    exact ⟨hVd.1, ih hVd.2 h₂⟩
+
+/-- Properties of reverse operation -/
+@[simp]
+lemma reverse_nil : (nil x : Walk α β).reverse = nil x := rfl
 
 @[simp]
-lemma first_eq_last_iff (hnodup : w.vx.Nodup) : w.first = w.last ↔ ¬ w.Nonempty := by
-  match w with
-  | .nil x => simp only [nil_first, nil_last, Nonempty.not_nil, not_false_eq_true]
-  | .cons x e w =>
-    simp only [cons_vx, nodup_cons, cons_first, cons_last, Nonempty.cons_true, not_true_eq_false,
-      iff_false, ne_eq] at hnodup ⊢
-    exact fun h => hnodup.1 (h ▸ last_vx_mem)
+lemma reverse_cons : (cons x e w).reverse = (w.reverse).concat e x := rfl
 
 @[simp]
-lemma first_ne_last_iff (hnodup : w.vx.Nodup) : w.first ≠ w.last ↔ w.Nonempty :=
-  (first_eq_last_iff hnodup).not_left
+lemma reverse_first : (reverse w).first = w.last := by
+  induction w with
+  | nil x => simp [reverse]
+  | cons x e w ih => simp [reverse, ih]
+
+@[simp]
+lemma reverse_last : (reverse w).last = w.first := by
+  induction w with
+  | nil x => simp [reverse]
+  | cons x e w ih => simp [reverse, ih]
+
+@[simp]
+lemma reverse_vx : (reverse w).vx = w.vx.reverse := by
+  induction w with
+  | nil x => simp [reverse]
+  | cons x e w ih => simp [reverse, ih]
+
+@[simp]
+lemma reverse_edge {w : Walk α β} : (reverse w).edge = w.edge.reverse := by
+  induction w with
+  | nil x => simp [reverse]
+  | cons x e w ih => simp [reverse, ih]
+
+@[simp]
+lemma reverse_length {w : Walk α β} : (reverse w).length = w.length := by
+  induction w with
+  | nil x => simp [reverse]
+  | cons x e w ih => simp [reverse, ih]
+
+lemma ValidIn.reverse (hVd : w.ValidIn G) : (reverse w).ValidIn G := by
+  induction w with
+  | nil x => simp [reverse, hVd]
+  | cons x e w ih =>
+    simp only [cons_validIn, reverse_cons] at hVd ⊢
+    refine ValidIn.concat (ih hVd.2) ?_
+    simp [hVd.1.symm]
+
+lemma IsWalkFrom.reverse (h : G.IsWalkFrom S T w) : G.IsWalkFrom T S w.reverse where
+  validIn := h.validIn.reverse
+  first_mem := by simp [h.last_mem]
+  last_mem := by simp [h.first_mem]
+
+lemma IsPath.reverse (hp : G.IsPath w) : G.IsPath w.reverse where
+  validIn := hp.validIn.reverse
+  nodup := by simp [hp.nodup]
+
+lemma IsPathFrom.reverse (p : G.IsPathFrom S T w) : G.IsPathFrom T S w.reverse where
+  validIn := p.validIn.reverse
+  nodup := by simp [p.nodup]
+  first_mem := by simp [p.last_mem]
+  last_mem := by simp [p.first_mem]
 
 /- Properties of append operation -/
 @[simp]
@@ -428,28 +424,25 @@ lemma append_validIn (h : w₁.last = w₂.first) (h₁ : w₁.ValidIn G) (h₂ 
     convert h₁.1 using 1
     exact append_first_of_eq h
 
-lemma ValidIn.append_left_validIn (h : w₁.last = w₂.first) (hw₁ : w₁.Nonempty)
+lemma ValidIn.append_left_validIn {w₁ w₂ : Walk α β} (h : w₁.last = w₂.first)
     (hVd : (w₁ ++ w₂).ValidIn G) : w₁.ValidIn G := by
-  induction w₁ with
-  | nil x => simp only [Nonempty.not_nil] at hw₁
-  | cons x e w ih =>
-    simp only [cons_append, cons_validIn_iff] at hVd
-    by_cases hNonempty : w.Nonempty
-    · refine ⟨?_, ih h hNonempty hVd.2⟩
-      convert hVd.1 using 1
-      simp only [hNonempty, append_first_of_nonempty]
-    · simp only [Nonempty.not_iff] at hNonempty
-      obtain ⟨y, rfl⟩ := hNonempty
-      simp only [cons_last, nil_last, nil_append, cons_validIn_iff, nil_first,
-        nil_validIn_iff] at h hVd ⊢
-      subst y
-      refine ⟨hVd.1, hVd.2.mem_of_mem_vx first_vx_mem⟩
+  match w₁ with
+  | .nil x =>
+    simp only [nil_last, nil_append, nil_validIn] at h hVd ⊢
+    subst x
+    exact hVd.vx_mem_of_mem first_mem
+  | .cons x e w =>
+    simp only [cons_last] at h
+    simp only [cons_append, cons_validIn] at hVd
+    refine ⟨?_, ValidIn.append_left_validIn h hVd.2⟩
+    convert hVd.1 using 1
+    exact (append_first_of_eq h).symm
 
 lemma ValidIn.append_right_validIn (hVd : (w₁ ++ w₂).ValidIn G) : w₂.ValidIn G := by
   induction w₁ with
   | nil x => simpa only [nil_append] using hVd
   | cons x e w ih =>
-    simp only [cons_append, cons_validIn_iff] at hVd
+    simp only [cons_append, cons_validIn] at hVd
     exact ih hVd.2
 
 lemma ValidIn.last_eq_first (hw₁ : w₁.Nonempty) (hVd₁ : w₁.ValidIn G) (hVd : (w₁ ++ w₂).ValidIn G) :
@@ -457,14 +450,54 @@ lemma ValidIn.last_eq_first (hw₁ : w₁.Nonempty) (hVd₁ : w₁.ValidIn G) (h
   induction w₁ with
   | nil x => simp only [Nonempty.not_nil] at hw₁
   | cons x e w ih =>
-    simp_all only [Nonempty.cons_true, cons_append, cons_validIn_iff, cons_last, forall_const]
+    simp_all only [Nonempty.cons_true, cons_append, cons_validIn, cons_last, forall_const]
     by_cases hNonempty : w.Nonempty
     · simp_all only [forall_const, append_first_of_eq, true_and]
     · simp only [Nonempty.not_iff] at hNonempty
       obtain ⟨y, rfl⟩ := hNonempty
-      simp_all only [Nonempty.not_nil, nil_last, IsEmpty.forall_iff, nil_first, nil_validIn_iff,
+      simp_all only [Nonempty.not_nil, nil_last, IsEmpty.forall_iff, nil_first, nil_validIn,
         nil_append]
       exact hVd₁.1.eq_of_inc₂ hVd.1
+
+lemma append_isWalkFrom (h : w₁.last = w₂.first) (h₁ : G.IsWalkFrom S T w₁)
+    (h₂ : G.IsWalkFrom T U w₂) : G.IsWalkFrom S U (w₁ ++ w₂) := by
+  obtain ⟨hw₁Vd, hw₁first, hw₁last⟩ := h₁
+  obtain ⟨hw₂Vd, hw₂first, hw₂last⟩ := h₂
+  refine ⟨?_, ?_, ?_⟩
+  · exact Walk.append_validIn h hw₁Vd hw₂Vd
+  · simpa [h]
+  · simpa
+
+lemma append_isPath (h : w₁.last = w₂.first) (h₁ : G.IsPath w₁) (h₂ : G.IsPath w₂)
+    (hvxSet : w₁.vxSet ∩ w₂.vxSet ⊆ {w₁.last}) : G.IsPath (w₁ ++ w₂) where
+  validIn := append_validIn h h₁.validIn h₂.validIn
+  nodup := by
+    simp only [Set.subset_singleton_iff, Set.mem_inter_iff, mem_vxSet_iff, and_imp, append_vx,
+      nodup_append, h₁.nodup.dropLast, h₂.nodup, true_and] at hvxSet ⊢
+    rintro x hx₁ hx₂
+    obtain rfl := hvxSet x (List.mem_of_mem_dropLast hx₁) hx₂
+    by_cases h : w₁.Nonempty
+    · rw [last_eq_vx_getLast] at hx₁
+      simp only [getLast_not_mem_dropLast_of_nodup h₁.nodup] at hx₁
+    · rw [Nonempty.not_iff] at h
+      obtain ⟨y, rfl⟩ := h
+      rw [nil_last] at h
+      subst y
+      simp at hx₁
+
+lemma append_left_isPath (h : w₁.last = w₂.first) (hP : G.IsPath (w₁ ++ w₂)) : G.IsPath w₁ where
+  validIn := hP.validIn.append_left_validIn h
+  nodup := by
+    have := hP.nodup
+    rw [append_vx' h] at this
+    exact this.of_append_left
+
+lemma append_right_isPath (hP : G.IsPath (w₁ ++ w₂)) : G.IsPath w₂ where
+  validIn := hP.validIn.append_right_validIn
+  nodup := by
+    have := hP.nodup
+    rw [append_vx] at this
+    exact this.of_append_right
 
 /- Properties of IsPrefix -/
 namespace IsPrefix
@@ -472,10 +505,20 @@ namespace IsPrefix
 instance instIsPrefixPreorder: IsPreorder (Walk α β) IsPrefix where
   refl w := ⟨nil w.last, by simp [append_nil rfl]⟩
   trans w1 w2 w3 h12 h23 := by
-    obtain ⟨w12, hw12⟩ := h12
-    obtain ⟨w23, hw23⟩ := h23
+    obtain ⟨w12, rfl, heq1⟩ := h12
+    obtain ⟨w23, rfl, heq2⟩ := h23
     use w23 ++ w12
-    rw [← append_assoc, ← hw23, ← hw12]
+    rw [← append_assoc, heq2]
+    rw [append_last] at heq1
+    simp only [heq1, append_first_of_eq, and_self]
+
+lemma ValidIn.IsPrefix (hPf : w.IsPrefix w₁) (hVd : w.ValidIn G) : w₁.ValidIn G := by
+  obtain ⟨w₂, rfl, heq⟩ := hPf
+  exact hVd.append_left_validIn heq
+
+lemma IsPath.IsPrefix (hPf : w.IsPrefix w₁) (hP : G.IsPath w) : G.IsPath w₁ := by
+  obtain ⟨w₂, rfl, heq⟩ := hPf
+  exact append_left_isPath heq hP
 
 end IsPrefix
 
@@ -484,272 +527,40 @@ namespace IsSuffix
 instance instIsSuffixPartialOrder: IsPartialOrder (Walk α β) IsSuffix where
   refl w := ⟨nil w.first, by simp [append_nil rfl]⟩
   trans w1 w2 w3 h12 h23 := by
-    obtain ⟨w12, hw12⟩ := h12
-    obtain ⟨w23, hw23⟩ := h23
+    obtain ⟨w12, rfl, heq1⟩ := h12
+    obtain ⟨w23, rfl, heq2⟩ := h23
+    simp only [heq2, append_first_of_eq] at heq1
     use w12 ++ w23
-    rw [append_assoc, ← hw23, ← hw12]
+    rw [← append_assoc]
+    simpa
   antisymm w1 w2 h12 h21 := by
-    obtain ⟨w21, hw21⟩ := h21
-    obtain ⟨w12, hw12⟩ := h12
+    obtain ⟨w21, hw21, heq21⟩ := h21
+    obtain ⟨w12, hw12, heq12⟩ := h12
     have := hw12 ▸ hw21 ▸ hw12
     rw [append_right_inj, ← append_assoc, eq_comm, append_left_eq_self] at this
     simp only [Nonempty.not_iff, append_eq_nil_iff, exists_and_left] at this
     obtain ⟨⟨y, rfl⟩, x, rfl⟩ := this
     simpa using hw12
 
+lemma ValidIn.IsSuffix (hPf : w.IsSuffix w₁) (hVd : w.ValidIn G) : w₁.ValidIn G := by
+  obtain ⟨w₂, rfl, heq⟩ := hPf
+  exact hVd.append_right_validIn
+
+lemma IsPath.IsSuffix (hPf : w.IsSuffix w₁) (hP : G.IsPath w) : G.IsPath w₁ := by
+  obtain ⟨w₂, rfl, heq⟩ := hPf
+  exact append_right_isPath hP
+
 end IsSuffix
-end Walk
-
-open Walk
-
-variable {G H : Graph α β} {u v : α} {e : β} {w : Walk α β}
-
-def Inc₂.walk (_h : G.Inc₂ e u v) : Walk α β := cons u e (nil v)
-
-lemma Inc₂.walk_validIn (h : G.Inc₂ e u v) : h.walk.ValidIn G := by
-  simp only [walk, ValidIn, h.vx_mem_right, nil_first, h, cons_validIn]
-
-@[simp] lemma Inc₂.Walk.first (h : G.Inc₂ e u v): h.walk.first = u := rfl
-
-@[simp] lemma Inc₂.Walk.last (h : G.Inc₂ e u v): h.walk.last = v := rfl
-
-@[simp] lemma Inc₂.Walk.vx (h : G.Inc₂ e u v): h.walk.vx = [u, v] := rfl
-
-@[simp] lemma Inc₂.Walk.edge (h : G.Inc₂ e u v): h.walk.edge = [e] := rfl
-
-@[simp] lemma Inc₂.Walk.length (h : G.Inc₂ e u v): h.walk.length = 1 := rfl
-
-@[simp] lemma Inc₂.Walk.mem_iff (h : G.Inc₂ e u v) (x : α) : x ∈ h.walk ↔ x = u ∨ x = v := by
-  simp [walk]
-
-lemma Inc₂.mem_left_of_edge_mem_walk (h : G.Inc₂ e u v) (he : e ∈ w.edge)
-    (hVd : w.ValidIn G) : u ∈ w := by
-  induction w with
-  | nil x => simp at he
-  | cons x e' w ih =>
-    simp only [cons_edge, mem_cons, cons_vx] at he ⊢
-    obtain rfl | he' := he
-    · obtain ⟨hbtw, hVd⟩ := hVd
-      obtain ⟨rfl, rfl⟩ | ⟨rfl, rfl⟩ := hbtw.eq_or_eq_of_inc₂ h
-      · left
-      · right
-        exact first_vx_mem
-    · right
-      exact ih he' hVd.2
-
-lemma Inc₂.mem_right_of_edge_mem_walk (h : G.Inc₂ e u v) (he : e ∈ w.edge)
-    (hVd : w.ValidIn G) : v ∈ w := h.symm.mem_left_of_edge_mem_walk he hVd
-
-/-- Given a graph adjacency, we can create a walk of length 1 -/
-lemma Adj.exist_walk (h : G.Adj u v) : ∃ (W : Walk α β), W.ValidIn G ∧ W.length = 1 ∧ W.first = u ∧
-    W.last = v := by
-  obtain ⟨e, he⟩ := h
-  use he.walk, he.walk_validIn
-  simp only [Inc₂.Walk.length, Inc₂.Walk.first, Inc₂.Walk.last, and_self]
-
-/-- Given a reflexive adjacency, we can create a walk of length at most 1 -/
-lemma reflAdj.exist_walk (h : G.reflAdj u v) : ∃ (W : Walk α β), W.ValidIn G ∧ W.length ≤ 1 ∧
-    W.first = u ∧ W.last = v := by
-  obtain hadj | ⟨rfl, hx⟩ := h
-  · obtain ⟨W, hW, hlength, hfirst, hlast⟩ := hadj.exist_walk
-    use W, hW
-    simp only [hlength, le_refl, hfirst, hlast, and_self]
-  · use nil u
-    constructor
-    · simp [hx]
-    · simp
-
-lemma Connected.exist_walk (h : G.Connected u v) : ∃ (W : Walk α β), W.ValidIn G ∧
-    W.first = u ∧ W.last = v := by
-  induction h with
-  | single hradj =>
-    obtain ⟨W, hW, hlength, hfirst, hlast⟩ := hradj.exist_walk
-    use W
-  | tail hconn hradj ih =>
-    expose_names
-    obtain ⟨W, hW, hfirst, hlast⟩ := ih
-    obtain ⟨W', hW', hlength, hfirst', hlast'⟩ := hradj.exist_walk
-    subst b c u
-    use W ++ W', append_validIn hfirst'.symm hW hW'
-    simp only [hfirst', append_first_of_eq, append_last, and_self]
-
-lemma Walk.connected_of_validIn (h : w.ValidIn G) : G.Connected w.first w.last := by
-  induction w with
-  | nil x => simpa only [nil_first, nil_last, Connected.refl_iff]
-  | cons x e w ih =>
-    obtain ⟨H1, H2⟩ := h
-    simp only [cons_first, cons_last]
-    exact H1.connected.trans (ih H2)
-
-lemma Walk.connected_of_validIn_of_mem' (h : w.ValidIn G) (hx : u ∈ w) :
-    G.Connected u w.last := by
-  induction w generalizing u with
-  | nil x =>
-    rw [mem_vx_nil_iff] at hx
-    subst u
-    simp only [nil_last, Connected.refl_iff]
-    exact h
-  | cons x e w ih =>
-    rw [mem_vx_cons_iff] at hx
-    obtain rfl | hx := hx
-    · exact Connected.trans h.1.connected (ih h.2 (first_vx_mem))
-    · exact ih h.2 hx
-
-lemma Walk.connected_of_validIn_of_mem (h : w.ValidIn G) (hx : x ∈ w) (hy : y ∈ w) :
-    G.Connected x y := by
-  have hx' := Walk.connected_of_validIn_of_mem' h hx
-  have hy' := Walk.connected_of_validIn_of_mem' h hy
-  exact Connected.trans hx' hy'.symm
-
-theorem Connected.iff_walk : G.Connected u v ↔ ∃ w : Walk α β, w.ValidIn G ∧ w.first = u ∧ w.last = v := by
-  constructor
-  · exact fun a ↦ exist_walk a
-  · rintro ⟨w, h1, rfl, rfl⟩
-    exact connected_of_validIn h1
-
-
-namespace Walk
-
-/-- Properties of dropLast operation -/
-@[simp]
-lemma dropLast_nil : (nil x : Walk α β).dropLast = nil x := rfl
-
-@[simp]
-lemma dropLast_cons_nil : (cons x e (nil y) : Walk α β).dropLast = nil x := rfl
-
-@[simp]
-lemma dropLast_cons_cons :
-  (cons x e (cons y e' w) : Walk α β).dropLast = cons x e ((cons y e' w).dropLast) := rfl
-
-@[simp]
-lemma dropLast_first {w : Walk α β} (h : w.Nonempty) : (w.dropLast).first = w.first := by
-  match w with
-  | .nil x => simp at h
-  | .cons x e (.nil y) => simp
-  | .cons x e (cons y e' w) => simp
-
-@[simp]
-lemma dropLast_vx {w : Walk α β} (h : w.Nonempty) : (w.dropLast).vx = w.vx.dropLast := by
-  match w with
-  | .nil x => simp only [Nonempty.not_nil] at h
-  | .cons x e (.nil y) => simp only [dropLast, nil_vx, cons_vx, dropLast_cons₂, dropLast_single]
-  | .cons x e (cons y e' w) =>
-    simp only [dropLast, cons_vx, dropLast_cons₂, List.cons.injEq, true_and]
-    rw [← cons_vx (e := e')]
-    apply dropLast_vx (by simp)
-
-@[simp]
-lemma dropLast_edge {w : Walk α β} (h : w.Nonempty) : (w.dropLast).edge = w.edge.dropLast := by
-  match w with
-  | .nil x => simp only [Nonempty.not_nil] at h
-  | .cons x e (.nil y) => simp only [dropLast, nil_edge, cons_edge, dropLast_single]
-  | .cons x e (cons y e' w) =>
-    simp only [dropLast, cons_edge, dropLast_cons₂, List.cons.injEq, true_and]
-    exact dropLast_edge (by simp)
-
-lemma dropLast_validIn {w : Walk α β} (hVd : w.ValidIn G) :
-    (w.dropLast).ValidIn G := by
-  match w with
-  | .nil x => simp only [dropLast, hVd]
-  | .cons x e (.nil y) =>
-    simp only [cons_validIn_iff, nil_first, nil_validIn_iff] at hVd
-    exact hVd.1.vx_mem_left
-  | .cons x e (cons y e' w) =>
-    rw [dropLast, cons_validIn_iff, dropLast_first (by simp)]
-    rw [cons_validIn_iff] at hVd
-    refine ⟨hVd.1, ?_⟩
-    exact dropLast_validIn hVd.2
-
-lemma mem_dropLast_or_last_of_mem {w : Walk α β} (hu : u ∈ w) :
-    u ∈ w.dropLast ∨ u = w.last := by
-  match w with
-  | .nil x => simpa using hu
-  | .cons x e (.nil y) =>
-    simp only [mem_vx_cons_iff, mem_vx_nil_iff] at hu
-    obtain rfl | rfl := hu <;> simp
-  | .cons x e (cons y e' w) =>
-    simp only [mem_vx_cons_iff] at hu
-    obtain rfl | rfl | hu := hu
-    · simp
-    · simp only [dropLast_cons_cons, mem_vx_cons_iff, cons_last]
-      have := mem_dropLast_or_last_of_mem (by simp : u ∈ (cons u e' w))
-      rw [cons_last] at this
-      tauto
-    · simp only [dropLast_cons_cons, mem_vx_cons_iff, cons_last]
-      have := mem_dropLast_or_last_of_mem (by simp [hu] : u ∈ (cons y e' w))
-      rw [cons_last] at this
-      tauto
-
-lemma mem_of_mem_dropLast {w : Walk α β} (h : u ∈ w.dropLast.vx) : u ∈ w := by
-  match w with
-  | .nil x => simpa using h
-  | .cons x e (.nil y) => simp_all only [dropLast_cons_nil, nil_vx, mem_cons, not_mem_nil, or_false,
-    mem_vx_cons_iff, mem_vx_nil_iff, true_or]
-  | .cons x e (cons y e' w) =>
-    simp only [dropLast_cons_cons, cons_vx, Nonempty.cons_true, dropLast_vx, mem_cons] at h ⊢
-    obtain rfl | h := h
-    · left
-    · have := mem_of_mem_dropLast (w := cons y e' w) (by simpa only [Nonempty.cons_true,
-      dropLast_vx, cons_vx])
-      right
-      simpa only [cons_vx, mem_cons] using this
-
-lemma mem_dropLast_or_last_of_mem_iff :
-    u ∈ w.dropLast ∨ u = w.last ↔ u ∈ w := by
-  refine ⟨?_, mem_dropLast_or_last_of_mem⟩
-  rintro (h | rfl)
-  · exact mem_of_mem_dropLast h
-  · exact last_vx_mem
-
-/-- Properties of concat operation -/
-@[simp]
-lemma concat_vx {w : Walk α β} {e : β} {v : α} : (w.concat e v).vx = w.vx ++ [v] := by
-  induction w with
-  | nil x => simp [concat]
-  | cons x e w ih => simp [concat, ih]
-
-@[simp]
-lemma concat_edge {w : Walk α β} {e : β} {v : α} : (w.concat e v).edge = w.edge ++ [e] := by
-  induction w with
-  | nil x => simp [concat]
-  | cons x e w ih => simp [concat, ih]
-
-@[simp]
-lemma concat_length {w : Walk α β} {e : β} {v : α} : (w.concat e v).length = w.length + 1 := by
-  induction w with
-  | nil x => simp [concat]
-  | cons x e w ih => simp [concat, ih]
-
-/-- Properties of reverse operation -/
-@[simp]
-lemma reverse_vx {w : Walk α β} : (reverse w).vx = w.vx.reverse := by
-  induction w with
-  | nil x => simp [reverse]
-  | cons x e w ih => simp [reverse, ih]
-
-@[simp]
-lemma reverse_edge {w : Walk α β} : (reverse w).edge = w.edge.reverse := by
-  induction w with
-  | nil x => simp [reverse]
-  | cons x e w ih => simp [reverse, ih]
-
-@[simp]
-lemma reverse_length {w : Walk α β} : (reverse w).length = w.length := by
-  induction w with
-  | nil x => simp [reverse]
-  | cons x e w ih => simp [reverse, ih]
-
-
 
 lemma eq_append_of_vx_mem {w : Walk α β} {u : α} (hmem : u ∈ w) :
     ∃ w₁ w₂ : Walk α β, w = w₁ ++ w₂ ∧ w₁.last = u ∧ w₂.first = u := by
   induction w with
   | nil x =>
-    rw [mem_vx_nil_iff] at hmem
+    rw [mem_nil_iff] at hmem
     subst u
     exact ⟨nil x, nil x, rfl, rfl, rfl⟩
   | cons x e w ih =>
-    rw [mem_vx_cons_iff] at hmem
+    rw [mem_cons_iff] at hmem
     obtain rfl | h := hmem
     · exact ⟨nil u, cons u e w, rfl, rfl, rfl⟩
     · obtain ⟨w₁, w₂, rfl, hfin, hfirst⟩ := ih h
@@ -771,57 +582,6 @@ lemma eq_append_cons_of_edge_mem {w : Walk α β} {e : β} (he : e ∈ w.edge) :
         use cons x e' w₁, w₂, by simp only [cons_last, cons_append]
         simp only [cons_edge, mem_cons, h, hnin, or_self, not_false_eq_true]
 
-/-- A subgraph inherits all valid walks -/
-lemma ValidIn.le {w : Walk α β} (h : w.ValidIn G) (hle : G ≤ H) : w.ValidIn H := by
-  match w with
-  | nil x => exact vx_subset_of_le hle h
-  | cons x e w =>
-    obtain ⟨hbtw, hVd⟩ := h
-    exact ⟨hbtw.le hle, hVd.le hle⟩
-
-lemma ValidIn.eq_nil_of_mem_isolated {w : Walk α β} {x : α} (hisol : G.Isolated x) (hmem : x ∈ w)
-    (h : w.ValidIn G) : w = nil x := by
-  match w with
-  | nil y => simp_all only [mem_vx_nil_iff, nil_validIn_iff]
-  | cons y e w =>
-    exfalso
-    obtain ⟨hbtw, hVd⟩ := h
-    rw [mem_vx_cons_iff] at hmem
-    obtain rfl | h := hmem
-    · exact hisol e hbtw.inc_left
-    · have := ValidIn.eq_nil_of_mem_isolated hisol h hVd
-      subst w
-      rw [nil_first] at hbtw
-      exact hisol e hbtw.inc_right
-
-lemma ValidIn.induce {U : Set α} (hVd : w.ValidIn G) (hU : ∀ x ∈ w, x ∈ U) : w.ValidIn (G[U]) := by
-  induction w with
-  | nil x => simp [hU]
-  | cons x e w ih =>
-    obtain ⟨hbtw, hVd⟩ := hVd
-    simp only [mem_vx_cons_iff, forall_eq_or_imp] at hU
-    obtain ⟨hUx, hUw⟩ := hU
-    refine ⟨?_, ih hVd hUw⟩
-    simp only [induce_inc₂_iff, hbtw, true_and, hUx]
-    exact hUw _ first_vx_mem
-
-lemma ValidIn.restrict {S : Set β} (hVd : w.ValidIn G) (hS : ∀ e ∈ w.edge, e ∈ S) :
-    w.ValidIn (G{S}) := by
-  induction w with
-  | nil x => exact hVd
-  | cons x e w ih =>
-    obtain ⟨hbtw, hVd⟩ := hVd
-    specialize ih hVd ?_
-    · rintro e' he'
-      refine hS e' ?_
-      simp only [cons_edge, mem_cons, he', or_true]
-    have he : e ∈ S := by
-      apply hS
-      simp only [cons_edge, mem_cons, true_or]
-    simp only [ih, restrict_inc₂, hbtw, he, and_self, cons_validIn]
-
-lemma ValidIn.subgraph {U : Set α} {S : Set β} (hVd : w.ValidIn G) (hU : ∀ x ∈ w, x ∈ U)
-    (hS : ∀ e ∈ w.edge, e ∈ S) : w.ValidIn (G{S}[U]) := ValidIn.induce (ValidIn.restrict hVd hS) hU
 
 end Walk
 -- noncomputable def Contract.walk {α' : Type*} {w : Walk α' β} {p : α → α'} {C : Set β}
@@ -894,6 +654,26 @@ end Walk
 --     -- change (w'.append (Walk.cons w'.last e <| walk hVd h.2 hbtw.vx_mem_right hy ha hpy)).ValidIn G
 --     sorry
 
+lemma Connected.exist_walk (h : G.Connected u v) : ∃ (W : Walk α β), W.ValidIn G ∧
+    W.first = u ∧ W.last = v := by
+  induction h with
+  | single hradj =>
+    obtain ⟨W, hW, hlength, hfirst, hlast⟩ := hradj.exist_walk
+    use W
+  | tail hconn hradj ih =>
+    expose_names
+    obtain ⟨W, hW, hfirst, hlast⟩ := ih
+    obtain ⟨W', hW', hlength, hfirst', hlast'⟩ := hradj.exist_walk
+    subst b c u
+    use W ++ W', append_validIn hfirst'.symm hW hW'
+    simp only [hfirst', append_first_of_eq, append_last, and_self]
+
+theorem Connected.iff_walk : G.Connected u v ↔ ∃ w : Walk α β, w.ValidIn G ∧ w.first = u ∧ w.last = v := by
+  constructor
+  · exact fun a ↦ exist_walk a
+  · rintro ⟨w, h1, rfl, rfl⟩
+    exact h1.connected
+
 lemma Contract.walk {α' : Type*} {w : Walk α' β} {p : α → α'} {C : Set β} (hVd : ValidIn G p C)
     (h : w.ValidIn (G /[p] C)) : ∀ x ∈ G.V, ∀ y ∈ G.V, p x = w.first → p y = w.last →
     ∃ w' : Walk α β, w'.ValidIn G ∧ w'.first = x ∧ w'.last = y ∧
@@ -908,7 +688,7 @@ lemma Contract.walk {α' : Type*} {w : Walk α' β} {p : α → α'} {C : Set β
     use w, ?_, rfl, rfl
     · simp only [nil_edge, not_mem_nil, false_or, setOf_mem_eq]
       rintro e he
-      have := hwVd.mem_of_mem_edge he
+      have := hwVd.edge_mem_of_mem he
       exact Set.mem_of_mem_inter_right this
     · exact hwVd.le (restrict_le _ _)
   | cons u e W ih =>
@@ -917,9 +697,9 @@ lemma Contract.walk {α' : Type*} {w : Walk α' β} {p : α → α'} {C : Set β
       apply ValidIn.restrict h ?_
       simp
     simp only [cons_first, cons_last] at hpx hpy
-    simp only [cons_edge, mem_cons, cons_validIn_iff, restrict_inc₂, Inc₂, mem_setOf_eq,
+    simp only [cons_edge, mem_cons, cons_validIn, restrict_inc₂, Inc₂, mem_setOf_eq,
       true_or, and_true] at hw
-    simp only [cons_validIn_iff, Inc₂] at h
+    simp only [cons_validIn, Inc₂] at h
     obtain ⟨⟨z, rfl, a, ha, hbtw, he⟩, hVdW⟩ := hw
     obtain ⟨_B, hVdWp⟩ := h
     rw [hVd hx hbtw.vx_mem_left] at hpx
@@ -929,7 +709,7 @@ lemma Contract.walk {α' : Type*} {w : Walk α' β} {p : α → α'} {C : Set β
     · simp +contextual only [append_edge, cons_edge, mem_append, mem_cons, setOf_subset_setOf]
       rintro f (hfw' | rfl | hfw)
       · right
-        have := hw'Vd.mem_of_mem_edge hfw'
+        have := hw'Vd.edge_mem_of_mem hfw'
         exact Set.mem_of_mem_inter_right this
       · tauto
       · obtain (h1 | h2) := hsu hfw <;> tauto
@@ -960,15 +740,15 @@ lemma Contract.map_walk_of_walk {α' : Type*} {w : Walk α β} {p : α → α'} 
         rintro f hfw'
         right
         exact hsub hfw'
-      · simp only [hw'Vd, cons_validIn_iff, Inc₂, and_true]
+      · simp only [hw'Vd, cons_validIn, Inc₂, and_true]
         use u, rfl, W.first, hst.symm, hbtw
 
 namespace Walk
 variable [DecidableEq α]
 
 @[simp]
-lemma firstAt_nil (hx : x ∈ (nil u : Walk α β).vx) : (nil u).firstAt x hx = nil x := by
-  simp only [nil_vx, mem_cons, not_mem_nil, or_false] at hx
+lemma firstAt_nil (hx : x ∈ (nil u : Walk α β)) : (nil u).firstAt x hx = nil x := by
+  simp only [mem_nil_iff] at hx
   subst u
   rfl
 
@@ -976,10 +756,10 @@ lemma firstAt_nil (hx : x ∈ (nil u : Walk α β).vx) : (nil u).firstAt x hx = 
 lemma firstAt_first (hx : x ∈ w) : (w.firstAt x hx).first = x := by
   induction w with
   | nil u =>
-    simp only [mem_vx_nil_iff] at hx
+    simp only [mem_nil_iff] at hx
     exact hx.symm
   | cons u e W ih =>
-    simp only [mem_vx_cons_iff] at hx
+    simp only [mem_cons_iff] at hx
     unfold firstAt
     by_cases h : x ∈ W
     · simp only [h, ↓reduceDIte]
@@ -992,7 +772,7 @@ lemma firstAt_last (hx : x ∈ w): (w.firstAt x hx).last = w.last := by
   induction w with
   | nil u => rfl
   | cons u e W ih =>
-    simp only [mem_vx_cons_iff] at hx
+    simp only [mem_cons_iff] at hx
     unfold firstAt
     by_cases h : x ∈ W
     · simp only [h, ↓reduceDIte, cons_last]
@@ -1004,7 +784,7 @@ lemma firstAt_length (hx : x ∈ w) : (w.firstAt x hx).length ≤ w.length := by
   induction w with
   | nil u => simp only [firstAt_nil, nil_length, le_refl]
   | cons u e W ih =>
-    simp only [mem_vx_cons_iff] at hx
+    simp only [mem_cons_iff] at hx
     unfold firstAt
     by_cases h : x ∈ W
     · simp only [h, ↓reduceDIte, cons_length]
@@ -1017,7 +797,7 @@ lemma firstAt_sizeOf_le (hx : x ∈ w) : sizeOf (w.firstAt x hx) ≤ sizeOf w :=
   induction w with
   | nil u => simp only [firstAt_nil, nil.sizeOf_spec, sizeOf_default, add_zero, le_refl]
   | cons u e W ih =>
-    rw [mem_vx_cons_iff] at hx
+    rw [mem_cons_iff] at hx
     unfold firstAt
     by_cases h : x ∈ W
     · simp only [h, ↓reduceDIte, cons.sizeOf_spec, sizeOf_default, add_zero]
@@ -1029,7 +809,7 @@ lemma firstAt_validIn (hx : x ∈ w) (hVd : w.ValidIn G) : (w.firstAt x hx).Vali
   induction w with
   | nil u => simpa [firstAt]
   | cons u e W ih =>
-    rw [mem_vx_cons_iff] at hx
+    rw [mem_cons_iff] at hx
     unfold firstAt
     by_cases h : x ∈ W
     · simp only [h, ↓reduceDIte]
@@ -1039,12 +819,12 @@ lemma firstAt_validIn (hx : x ∈ w) (hVd : w.ValidIn G) : (w.firstAt x hx).Vali
 lemma firstAt_vx_count (hx : x ∈ w) : (w.firstAt x hx).vx.count x = 1 := by
   induction w with
   | nil u =>
-    rw [mem_vx_nil_iff] at hx
+    rw [mem_nil_iff] at hx
     subst u
     unfold firstAt
     simp
   | cons u e W ih =>
-    rw [mem_vx_cons_iff] at hx
+    rw [mem_cons_iff] at hx
     unfold firstAt
     by_cases h : x ∈ W
     · simp only [h, ↓reduceDIte]
@@ -1057,12 +837,12 @@ lemma firstAt_vx_count (hx : x ∈ w) : (w.firstAt x hx).vx.count x = 1 := by
 lemma firstAt_isSuffix (hx : x ∈ w) : ∃ w' : Walk α β, w' ++ (w.firstAt x hx) = w := by
   induction w generalizing x with
   | nil u =>
-    rw [mem_vx_nil_iff] at hx
+    rw [mem_nil_iff] at hx
     subst u
     use nil x
     rfl
   | cons u e W ih =>
-    rw [mem_vx_cons_iff] at hx
+    rw [mem_cons_iff] at hx
     unfold firstAt
     by_cases h : x ∈ W
     · simp only [h, ↓reduceDIte]
@@ -1076,11 +856,11 @@ lemma firstAt_isSuffix (hx : x ∈ w) : ∃ w' : Walk α β, w' ++ (w.firstAt x 
 lemma firstAt_vx_sublist (hx : x ∈ w) : (w.firstAt x hx).vx ⊆ w.vx := by
   induction w with
   | nil u =>
-    rw [mem_vx_nil_iff] at hx
+    rw [mem_nil_iff] at hx
     subst u
     simp only [firstAt_nil, nil_vx, List.Subset.refl]
   | cons u e W ih =>
-    rw [mem_vx_cons_iff] at hx
+    rw [mem_cons_iff] at hx
     unfold firstAt
     by_cases h : x ∈ W
     · simp only [h, ↓reduceDIte, cons_vx]
@@ -1091,11 +871,11 @@ lemma firstAt_vx_sublist (hx : x ∈ w) : (w.firstAt x hx).vx ⊆ w.vx := by
 lemma firstAt_edge_sublist (hx : x ∈ w) : (w.firstAt x hx).edge ⊆ w.edge := by
   induction w with
   | nil u =>
-    rw [mem_vx_nil_iff] at hx
+    rw [mem_nil_iff] at hx
     subst u
     simp only [firstAt_nil, nil_edge, List.Subset.refl]
   | cons u e W ih =>
-    rw [mem_vx_cons_iff] at hx
+    rw [mem_cons_iff] at hx
     unfold firstAt
     by_cases h : x ∈ W
     · simp only [h, ↓reduceDIte, cons_edge]
@@ -1168,11 +948,11 @@ lemma dedup_validIn {w : Walk α β} (hVd : w.ValidIn G) : w.dedup.ValidIn G := 
     split_ifs with h
     · simp only [h, ↓reduceDIte]
       exact dedup_validIn (firstAt_validIn h hVd.2)
-    · simp only [dedup_validIn hVd.2, cons_validIn_iff, and_true]
+    · simp only [dedup_validIn hVd.2, cons_validIn, and_true]
       convert hVd.1 using 1
       exact dedup_first W
 
-lemma dedup_vx_sublist {w : Walk α β} {x : α} (hx : x ∈ w.dedup.vx) : x ∈ w := by
+lemma dedup_vx_sublist {w : Walk α β} {x : α} (hx : x ∈ w.dedup) : x ∈ w := by
   match w with
   | .nil u =>
     unfold dedup at hx
@@ -1182,7 +962,7 @@ lemma dedup_vx_sublist {w : Walk α β} {x : α} (hx : x ∈ w.dedup.vx) : x ∈
     split_ifs at hx with h
     · simp only at hx
       exact mem_of_mem_tail <| firstAt_vx_sublist h <| dedup_vx_sublist hx
-    · simp only [cons_vx, mem_cons, mem_notation, mem_vx_cons_iff] at hx ⊢
+    · simp only [cons_vx, mem_cons, mem_notation, mem_cons_iff] at hx ⊢
       exact hx.imp (·) dedup_vx_sublist
 
 lemma dedup_edge_sublist (w : Walk α β) : w.dedup.edge ⊆ w.edge := by
@@ -1269,7 +1049,7 @@ lemma endIf_last {w : Walk α β} (h : ∃ u ∈ w, P u) : P (w.endIf h).last :=
     rw [endIf]
     split_ifs with hPx
     · simpa only [nil_last]
-    · simp only [mem_vx_cons_iff, exists_eq_or_imp, hPx, false_or, cons_last] at h ⊢
+    · simp only [mem_cons_iff, exists_eq_or_imp, hPx, false_or, cons_last] at h ⊢
       exact endIf_last h
 
 @[simp]
@@ -1314,17 +1094,17 @@ lemma endIf_sizeOf_le {w : Walk α β} (h : ∃ u ∈ w, P u) :
 lemma endIf_validIn {w : Walk α β} (h : ∃ u ∈ w, P u) (hVd : w.ValidIn G) :
     (w.endIf h).ValidIn G := by
   match w with
-  | .nil x => simpa only [endIf, nil_validIn_iff]
+  | .nil x => simpa only [endIf, nil_validIn]
   | .cons x e w =>
     simp only [endIf]
     split_ifs with hPx
-    · rw [nil_validIn_iff]
-      simp only [cons_validIn_iff] at hVd
+    · rw [nil_validIn]
+      simp only [cons_validIn] at hVd
       exact hVd.1.vx_mem_left
-    · rw [cons_validIn_iff] at hVd ⊢
+    · rw [cons_validIn] at hVd ⊢
       refine ⟨?_, endIf_validIn _ hVd.2⟩
       convert hVd.1 using 1
-      simp only [mem_vx_cons_iff, exists_eq_or_imp, hPx, false_or] at h
+      simp only [mem_cons_iff, exists_eq_or_imp, hPx, false_or] at h
       exact endIf_first h
 
 lemma endIf_vx_sublist {w : Walk α β} (h : ∃ u ∈ w, P u) :
@@ -1340,24 +1120,22 @@ lemma endIf_vx_sublist {w : Walk α β} (h : ∃ u ∈ w, P u) :
       refine List.Subset.trans ?_ (List.subset_cons_self _ _)
       apply endIf_vx_sublist
 
-lemma endIf_mem_vx {w : Walk α β} (h : ∃ u ∈ w, P u) (hv : v ∈ (w.endIf h).vx):
+lemma endIf_mem_vx {w : Walk α β} (h : ∃ u ∈ w, P u) (hv : v ∈ w.endIf h):
     ¬ P v ∨ v = (w.endIf h).last := by
   match w with
-  | .nil x => simp_all only [endIf_nil, nil_vx, mem_cons, not_mem_nil, or_false, nil_last,
-    or_true]
+  | .nil x => simp_all only [endIf_nil, mem_nil_iff, nil_last, or_true]
   | .cons x e w =>
     rw [endIf_cons]
     split_ifs with hPx
-    · simp_all only [endIf_cons, dite_true, nil_vx, mem_cons, not_mem_nil, or_false,
-      not_true_eq_false, nil_last, or_true]
-    · simp_all only [endIf_cons, dite_false, cons_vx, mem_cons, cons_last]
+    · simp_all only [endIf_cons, dite_true, mem_nil_iff, not_true_eq_false, nil_last, or_true]
+    · simp_all only [endIf_cons, dite_false, mem_cons_iff, cons_last]
       obtain rfl | hvmem := hv
       · exact Or.inl hPx
-      · simp only [mem_vx_cons_iff, exists_eq_or_imp, hPx, false_or] at h
+      · simp only [mem_cons_iff, exists_eq_or_imp, hPx, false_or] at h
         exact endIf_mem_vx h hvmem
 
 lemma endIf_dropLast_mem_vx {w : Walk α β} (h : ∃ u ∈ w, P u) (hNonempty : (w.endIf h).Nonempty)
-    (hu : u ∈ (w.endIf h).dropLast.vx) : ¬ P u := by
+    (hu : u ∈ (w.endIf h).dropLast) : ¬ P u := by
   match w with
   | .nil x => simp_all only [endIf_nil, Nonempty.not_nil]
   | .cons x e (nil y) =>
@@ -1365,24 +1143,23 @@ lemma endIf_dropLast_mem_vx {w : Walk α β} (h : ∃ u ∈ w, P u) (hNonempty :
     split_ifs at hu with hPx
     · simp_all only [cons_vx, nil_vx, mem_cons, not_mem_nil, or_false, exists_eq_or_imp,
       exists_eq_left, true_or, ite_true, Nonempty.not_nil]
-    · simp_all only [cons_vx, nil_vx, mem_cons, not_mem_nil, or_false, exists_eq_or_imp,
-      exists_eq_left, false_or, ite_false, Nonempty.cons_true, dropLast_cons₂, dropLast_single,
-      not_false_eq_true]
+    · simp_all only [mem_cons_iff, mem_nil_iff, exists_eq_or_imp, exists_eq_left, false_or,
+      ite_false, Nonempty.cons_true, dropLast_cons_nil, not_false_eq_true]
   | .cons x e (cons y e' w) =>
     by_cases hPx : P x
     · simp_all
     · by_cases hxu : u = x
       · simp_all
       · obtain ⟨v, hv, hv2⟩ := h
-        rw [mem_vx_cons_iff] at hv
+        rw [mem_cons_iff] at hv
         obtain rfl | hvmem := hv
         · simp_all
         · have hexists : ∃ u ∈ (cons y e' w), P u := by use v
           by_cases hnonempty : ((cons y e' w).endIf hexists).Nonempty
           · refine endIf_dropLast_mem_vx (w := cons y e' w) (by use v) hnonempty ?_
             by_cases hPy : P y
-            · simp only [endIf_cons, hPx, ↓reduceDIte, hPy, dropLast_cons_nil, nil_vx, mem_cons,
-                hxu, not_mem_nil, or_self] at hu
+            · simp only [endIf_cons, hPx, ↓reduceDIte, hPy, dropLast_cons_nil, mem_nil_iff,
+              hxu] at hu
             · simpa [hPx, hPy, hxu] using hu
           · simp only [Nonempty.not_iff] at hnonempty
             obtain ⟨a, ha⟩ := hnonempty
@@ -1393,11 +1170,11 @@ lemma endIf_exists_inc₂_last {w : Walk α β} (h : ∃ u ∈ w, P u) (hVd : w.
   match w with
   | .nil x => simp_all only [endIf_nil, Nonempty.not_nil]
   | .cons x e (nil y) =>
-    simp_all only [cons_validIn_iff, nil_first, nil_validIn_iff, endIf_cons, endIf_nil, dite_eq_ite]
+    simp_all only [cons_validIn, nil_first, nil_validIn, endIf_cons, endIf_nil, dite_eq_ite]
     split_ifs with hPx
     · simp_all only [cons_vx, nil_vx, mem_cons, not_mem_nil, or_false, exists_eq_or_imp,
       exists_eq_left, true_or, ite_true, Nonempty.not_nil]
-    · simp_all only [mem_vx_cons_iff, mem_vx_nil_iff, exists_eq_or_imp, exists_eq_left, false_or,
+    · simp_all only [mem_cons_iff, mem_nil_iff, exists_eq_or_imp, exists_eq_left, false_or,
       ite_false, Nonempty.cons_true, cons_last, nil_last, not_false_eq_true, true_and,
       not_true_eq_false, false_and, or_false]
       use e
@@ -1405,29 +1182,28 @@ lemma endIf_exists_inc₂_last {w : Walk α β} (h : ∃ u ∈ w, P u) (hVd : w.
   | .cons x e (cons y e' w) =>
     unfold endIf
     split_ifs with hPx
-    · simp_all only [cons_validIn_iff, cons_first, endIf_cons, dite_true, Nonempty.not_nil]
+    · simp_all only [cons_validIn, cons_first, endIf_cons, dite_true, Nonempty.not_nil]
     · by_cases hPy : P y
-      · simp_all only [cons_validIn_iff, cons_first, endIf_cons, dite_true, dite_eq_ite, ite_false,
-        Nonempty.cons_true, mem_vx_cons_iff, mem_vx_nil_iff, cons_last, nil_last,
+      · simp_all only [cons_validIn, cons_first, endIf_cons, dite_true, dite_eq_ite, ite_false,
+        Nonempty.cons_true, mem_cons_iff, mem_nil_iff, cons_last, nil_last,
         exists_eq_or_imp, not_false_eq_true, true_and, exists_eq_left, not_true_eq_false, false_and,
         or_false]
         use e
         exact hVd.1
       · let w' := cons y e' w
         rw [cons_last]
-        have h' : ∃ u ∈ w'.vx, P u := by
-          change ∃ u ∈ (cons x e w').vx, P u at h
-          simpa only [cons_vx, mem_cons, exists_eq_or_imp, hPx, false_or] using h
+        have h' : ∃ u ∈ w', P u := by
+          change ∃ u ∈ cons x e w', P u at h
+          simpa only [mem_cons_iff, exists_eq_or_imp, hPx, false_or] using h
         have hNonempty' : (w'.endIf h').Nonempty := by
           simp only [endIf_cons, hPy, ↓reduceDIte, Nonempty.cons_true, w']
         obtain ⟨a, ha, hh⟩ := endIf_exists_inc₂_last (w := w') h' hVd.2 hNonempty'
         refine ⟨a, ?_, hh⟩
-        rw [mem_vx_cons_iff]
+        rw [mem_cons_iff]
         right
         exact ha
 
 end Walk
-
 
 noncomputable def dist {G : Graph α β} {u v : α} (h : G.Connected u v) : ℕ := by
   classical
