Kura/Separators.lean
@@ -1,9 +1,11 @@
 import Kura.Operation.Subgraph
-import Kura.Walk.Walk
+import Kura.Walk.Operation
 
-open Set Function
-variable {α β : Type*} {G G₁ G₂ : Graph α β} {u v w x y z : α} {e f g : β}
+
 namespace Graph
+open Set Function List Nat Walk
+variable {α β : Type*} {G G' H H' : Graph α β} {u v x y z : α} {e e' f g : β} {S T U: Set α}
+  {F F' : Set β} {w w1 w2 : Walk α β}
 
 
 @[mk_iff]
@@ -50,7 +52,7 @@ lemma isVxSetSeparator_iff_inter_vxSet (G : Graph α β) {V S T : Set α} :
     G.IsVxSetSeparator V S T ↔ G.IsVxSetSeparator V (S ∩ G.V) (T ∩ G.V) := sorry
 
 @[simp]
-lemma le (h : G₂.IsVxSetSeparator V S T) (hle : G₁ ≤ G₂) : G₁.IsVxSetSeparator V S T := by
+lemma le (h : G'.IsVxSetSeparator V S T) (hle : G ≤ G') : G.IsVxSetSeparator V S T := by
   rintro s hs t ht hconn
   refine h s hs t ht (hconn.le (induce_le_induce hle ?_))
   exact Set.diff_subset_diff_left hle.1
@@ -266,127 +268,124 @@ def of_edges (G : Graph α β) (U : Set β) :
   sorry
 
 
-lemma path_inter {p : Path α β} (hUsep : G.IsVxSetSeparator U S T) (hVd : p.val.ValidOn G)
-    (hS : p.val.start ∈ S) (hT : p.val.finish ∈ T) : ∃ x ∈ p.val.vx, x ∈ U := by
+lemma walk_inter (hUsep : G.IsVxSetSeparator U S T) (hVd : w.ValidIn G)
+    (hS : w.first ∈ S) (hT : w.last ∈ T) : ∃ x ∈ w, x ∈ U := by
   by_contra! hx
-  have hVdU : p.val.ValidOn (G - U) := by
-    refine ValidOn.induce hVd ?_
-    rintro x hxp
-    exact ⟨hVd.mem_of_mem_vx hxp, hx x hxp⟩
-  exact hUsep p.val.start hS p.val.finish hT <| Walk.connected_of_validOn hVdU
+  have hVdU : w.ValidIn (G - U) := ValidIn.vxDel hVd fun V hV hVU x hxV ↦ hx x (hV hxV) (hVU hxV)
+  exact hUsep w.first hS w.last hT hVdU.connected
 
-lemma walk_validOn_left (hUsep : G.IsVxSetSeparator U S T) (hVd : w.ValidOn (G - U))
-    (hLeft : ∃ x ∈ w.vx, x ∈ hUsep.leftSet) : w.ValidOn (G[hUsep.leftSet]) := by
+lemma walk_validOn_left (hUsep : G.IsVxSetSeparator U S T) (hVd : w.ValidIn (G - U))
+    (hLeft : ∃ x ∈ w, x ∈ hUsep.leftSet) : w.ValidIn (G[hUsep.leftSet]) := by
   obtain ⟨y, hy, s, hs, hys⟩ := hLeft
   refine hVd.le (induce_le G diff_subset) |>.induce fun x hxp ↦ ?_
-  use s, hs, (w.connected_of_validOn_of_mem hVd hxp hy).trans hys
+  use s, hs, (hVd.connected_of_mem hxp hy).trans hys
 
-lemma walk_validOn_right (hUsep : G.IsVxSetSeparator U S T) (hVd : w.ValidOn (G - U))
-    (hT : ∃ x ∈ w.vx, x ∈ hUsep.rightSet) :
-    w.ValidOn (G[hUsep.rightSet]) := by
+lemma walk_validOn_right (hUsep : G.IsVxSetSeparator U S T) (hVd : w.ValidIn (G - U))
+    (hT : ∃ x ∈ w, x ∈ hUsep.rightSet) :
+    w.ValidIn (G[hUsep.rightSet]) := by
   obtain ⟨y, hy, s, hs, hys⟩ := hT
   refine hVd.le (induce_le G diff_subset) |>.induce fun x hxp ↦ ?_
-  use s, hs, (w.connected_of_validOn_of_mem hVd hxp hy).trans hys
+  use s, hs, (hVd.connected_of_mem hxp hy).trans hys
 
-lemma path_in_leftHalf_of_finishSep {w : Walk α β} (hNodup : w.vx.Nodup) (hVd : w.ValidOn G)
-    (hUsep : G.IsVxSetSeparator {w.finish} S T) (hS : w.start ∈ hUsep.leftSet) (hx : x ∈ w.vx) :
-    x ∈ hUsep.leftSet ∪ {w.finish} := by
+lemma path_in_leftHalf_of_finishSep {w : Walk α β} (hNodup : w.vx.Nodup) (hVd : w.ValidIn G)
+    (hUsep : G.IsVxSetSeparator {w.last} S T) (hS : w.first ∈ hUsep.leftSet) (hx : x ∈ w.vx) :
+    x ∈ hUsep.leftSet ∪ {w.last} := by
   obtain (h | h) := em (w.Nonempty) |>.symm
   · right
     rw [Nonempty.not_iff] at h
     obtain ⟨y, hy⟩ := h
-    simpa only [hy, nil_finish, mem_singleton_iff, nil_vx, mem_cons, not_mem_nil, or_false] using hx
+    simpa only [hy, nil_last, mem_singleton_iff, nil_vx, mem_cons, not_mem_nil, or_false] using hx
   rw [Nonempty.iff_exists_cons] at h
   obtain ⟨y, e, w', rfl⟩ := h
   simp only [cons_vx, mem_cons] at hx
   obtain (rfl | hx) := hx
   · left
-    simpa only [cons_finish, cons_start] using hS
+    simpa only [cons_last, cons_first] using hS
   · unfold leftSet
-    simp only [cons_finish] at hUsep ⊢
-    change x ∈ hUsep.leftSet ∪ {w'.finish}
-    by_cases hw' : w'.start = w'.finish
+    simp only [cons_last] at hUsep ⊢
+    change x ∈ hUsep.leftSet ∪ {w'.last}
+    by_cases hw' : w'.first = w'.last
     · simp [cons_vx_nodup hNodup] at hw'
       obtain ⟨y, rfl⟩ := hw'
       right
       simpa using hx
-    · apply (path_in_leftHalf_of_finishSep (w := w') (cons_vx_nodup hNodup) hVd.of_cons hUsep · hx)
-      simp only [cons_finish, cons_start] at hS
+    · apply (path_in_leftHalf_of_finishSep (w := w') (cons_vx_nodup hNodup) hVd.cons hUsep · hx)
+      simp only [cons_last, cons_first] at hS
       obtain ⟨s, hs, hys⟩ := hS
       use s, hs, Connected.trans ?_ hys
       refine (hVd.1.induce_of_mem hys.mem_left ?_).connected.symm
-      refine ⟨hVd.2.mem_of_mem_vx start_vx_mem, hw'⟩
+      refine ⟨hVd.2.vx_mem_of_mem first_mem, hw'⟩
 
-lemma path_validOn_leftHalf_of_finishSep (hUsep : G.IsVxSetSeparator {p.val.finish} S T)
-    (hVd : p.val.ValidOn G) (hS : p.val.start ∈ hUsep.leftSet) :
-    p.val.ValidOn (G[hUsep.leftSet ∪ {p.val.finish}]) :=
-  hVd.induce <| fun _ => path_in_leftHalf_of_finishSep (w := p.val) p.prop hVd hUsep hS
+lemma path_validOn_leftHalf_of_finishSep (hUsep : G.IsVxSetSeparator {w.last} S T) (hNodup : w.vx.Nodup)
+    (hVd : w.ValidIn G) (hS : w.first ∈ hUsep.leftSet) :
+    w.ValidIn (G[hUsep.leftSet ∪ {w.last}]) :=
+  hVd.induce <| fun _ => path_in_leftHalf_of_finishSep (w := w) hNodup hVd hUsep hS
 
 instance IsPreorder : IsPreorder (Set α) (IsVxSetSeparator G · S ·) where
   refl A s hs a ha hconn := by
     have := hconn.mem_right
     simp only [vxDel_V, mem_diff, ha, not_true_eq_false, and_false] at this
   trans A B C hAB hBC s hs c hc hconn := by
-    rw [Connected.iff_path] at hconn
+    rw [Connected.iff_walk] at hconn
     obtain ⟨p, hpVd, rfl, rfl⟩ := hconn
-    obtain ⟨x, hxp, hxB⟩ := hBC.path_inter (hpVd.le (induce_le G Set.diff_subset)) hs hc
-    exact hAB p.val.start hs x hxB <| p.val.connected_of_validOn_of_mem hpVd start_vx_mem hxp
+    obtain ⟨x, hxp, hxB⟩ := hBC.walk_inter (hpVd.le (induce_le G Set.diff_subset)) hs hc
+    exact hAB p.first hs x hxB <| hpVd.connected_of_mem first_mem hxp
 
 lemma crossingWalk_intersect (hVsep : G.IsVxSetSeparator V S T) [DecidablePred (· ∈ V)]
-    {w : Walk α β} (hwVd : w.ValidOn G) (hwstart : w.start ∈ hVsep.leftSet ∪ V)
-    (hwfinish : w.finish ∈ hVsep.rightSet ∪ V) : ∃ x ∈ w.vx, x ∈ V := by
-  rw [mem_union] at hwstart hwfinish
-  obtain (hV | ⟨s, hs, hconnStart⟩) := hwstart.symm <;> clear hwstart
-  · use w.start, start_vx_mem
-  obtain (hV | ⟨t, ht, hconnFinish⟩) := hwfinish.symm <;> clear hwfinish
-  · use w.finish, finish_vx_mem
+    (hwVd : w.ValidIn G) (hwfirst : w.first ∈ hVsep.leftSet ∪ V)
+    (hwlast : w.last ∈ hVsep.rightSet ∪ V) : ∃ x ∈ w.vx, x ∈ V := by
+  rw [mem_union] at hwfirst hwlast
+  obtain (hV | ⟨s, hs, hconnStart⟩) := hwfirst.symm <;> clear hwfirst
+  · use w.first, first_mem
+  obtain (hV | ⟨t, ht, hconnFinish⟩) := hwlast.symm <;> clear hwlast
+  · use w.last, last_mem
   by_contra! hw
-  have hVd : w.ValidOn (G - V) :=
-    hwVd.induce fun x hx ↦ ⟨hwVd.mem_of_mem_vx hx, hw x hx⟩
-  exact hVsep s hs t ht <| hconnStart.symm.trans (w.connected_of_validOn hVd) |>.trans hconnFinish
+  have hVd : w.ValidIn (G - V) :=
+    hwVd.induce fun x hx ↦ ⟨hwVd.vx_mem_of_mem hx, hw x hx⟩
+  exact hVsep s hs t ht <| hconnStart.symm.trans hVd.connected |>.trans hconnFinish
 
 lemma crossingWalk_intersect' (hVsep : G.IsVxSetSeparator V S T) [DecidablePred (· ∈ V)]
-    {w : Walk α β} (hwVd : w.ValidOn G) (hwstart : w.start ∈ hVsep.rightSet ∪ V)
-    (hwfinish : w.finish ∈ hVsep.leftSet ∪ V) : ∃ x ∈ w.vx, x ∈ V :=
-  crossingWalk_intersect hVsep.symm hwVd hwstart hwfinish
+    {w : Walk α β} (hwVd : w.ValidIn G) (hwfirst : w.first ∈ hVsep.rightSet ∪ V)
+    (hwlast : w.last ∈ hVsep.leftSet ∪ V) : ∃ x ∈ w.vx, x ∈ V :=
+  crossingWalk_intersect hVsep.symm hwVd hwfirst hwlast
 
 lemma crossingWalk_endIf_validOn [DecidableEq α] (hVsep : G.IsVxSetSeparator V S T)
-    [DecidablePred (· ∈ V)] {w : Walk α β} (hwVd : w.ValidOn G)
-    (hwstart : w.start ∈ hVsep.leftSet ∪ V) (hwfinish : w.finish ∈ hVsep.rightSet ∪ V) :
+    [DecidablePred (· ∈ V)] {w : Walk α β} (hwVd : w.ValidIn G)
+    (hwfirst : w.first ∈ hVsep.leftSet ∪ V) (hwlast : w.last ∈ hVsep.rightSet ∪ V) :
     (w.endIf (P := (· ∈ V))
-    (hVsep.crossingWalk_intersect hwVd hwstart hwfinish)).ValidOn (G[hVsep.leftSet ∪ V]) := by
-  let h := hVsep.crossingWalk_intersect hwVd hwstart hwfinish
-  refine endIf_validOn h hwVd |>.induce ?_
+    (hVsep.crossingWalk_intersect hwVd hwfirst hwlast)).ValidIn (G[hVsep.leftSet ∪ V]) := by
+  let h := hVsep.crossingWalk_intersect hwVd hwfirst hwlast
+  refine endIf_validIn h hwVd |>.induce ?_
   rintro x hx
   by_cases hnonempty : ¬ (w.endIf h).Nonempty
   · rw [Nonempty.not_iff] at hnonempty
     obtain ⟨y, hy⟩ := hnonempty
-    simp only [hy, nil_vx, mem_cons, not_mem_nil, or_false] at hx
+    simp only [hy, nil_vxSet, mem_singleton_iff] at hx
     subst y
     right
-    convert endIf_finish h
-    simp only [hy, nil_finish]
+    convert endIf_last h
+    simp only [hy, nil_last]
   rw [not_not] at hnonempty
-  obtain (rfl | hxV) := mem_dropLast_or_finish_of_mem hx |>.symm
+  obtain (rfl | hxV) := mem_dropLast_or_last_of_mem hx |>.symm
   · right
-    exact endIf_finish h
-  · have := dropLast_validOn (endIf_validOn h hwVd)
-    have : Walk.ValidOn _ (G - V):= this.induce fun x hx ↦
-      ⟨this.mem_of_mem_vx hx, endIf_dropLast_mem_vx h hnonempty hx⟩
+    exact endIf_last h
+  · have := dropLast_validIn (endIf_validIn h hwVd)
+    have : Walk.ValidIn _ (G - V):= this.induce fun x hx ↦
+      ⟨this.vx_mem_of_mem hx, endIf_dropLast_mem_vx h hnonempty hx⟩
     simp only [endIf_nonempty_iff] at hnonempty
-    simp only [mem_union, hnonempty, or_false] at hwstart
+    simp only [mem_union, hnonempty, or_false] at hwfirst
     left
-    refine (hVsep.walk_validOn_left this ?_).mem_of_mem_vx hxV
-    use w.start, ?_
-    convert start_vx_mem using 1
-    simp only [endIf_nonempty_iff, hnonempty, not_false_eq_true, dropLast_start, endIf_start]
+    refine (hVsep.walk_validOn_left this ?_).vx_mem_of_mem hxV
+    use w.first, ?_
+    convert first_mem using 1
+    simp [endIf_nonempty_iff, hnonempty, not_false_eq_true, dropLast_first, endIf_first]
 
 lemma crossingWalk_endIf_validOn' [DecidableEq α] [DecidablePred (· ∈ V)]
     (hVsep : G.IsVxSetSeparator V S T)
-    {w : Walk α β} (hwVd : w.ValidOn G) (hwstart : w.start ∈ hVsep.rightSet ∪ V)
-    (hwfinish : w.finish ∈ hVsep.leftSet ∪ V) : (w.endIf (P := (· ∈ V))
-    (hVsep.crossingWalk_intersect' hwVd hwstart hwfinish)).ValidOn (G[hVsep.rightSet ∪ V]) :=
-  hVsep.symm.crossingWalk_endIf_validOn hwVd hwstart hwfinish
+    (hwVd : w.ValidIn G) (hwfirst : w.first ∈ hVsep.rightSet ∪ V)
+    (hwlast : w.last ∈ hVsep.leftSet ∪ V) : (w.endIf (P := (· ∈ V))
+    (hVsep.crossingWalk_intersect' hwVd hwfirst hwlast)).ValidIn (G[hVsep.rightSet ∪ V]) :=
+  hVsep.symm.crossingWalk_endIf_validOn hwVd hwfirst hwlast
 
 lemma leftSetV_iff (h : G.IsVxSetSeparator V S T) (hV : V ⊆ G.V) (U : Set α) :
     G[h.leftSet ∪ V].IsVxSetSeparator U S V ↔ G.IsVxSetSeparator U S V := by
@@ -395,25 +394,25 @@ lemma leftSetV_iff (h : G.IsVxSetSeparator V S T) (hV : V ⊆ G.V) (U : Set α) 
   · rintro hUsep s hs v hv hconn
     rw [Connected.iff_walk] at hconn
     obtain ⟨w, hwVd, rfl, rfl⟩ := hconn
-    have hwVdG : w.ValidOn G := hwVd.le (induce_le _ Set.diff_subset)
-    have hwstart : w.start ∈ h.leftSet ∪ V := by
-      by_cases hsUv : w.start ∈ V
+    have hwVdG : w.ValidIn G := hwVd.le (induce_le _ Set.diff_subset)
+    have hwfirst : w.first ∈ h.leftSet ∪ V := by
+      by_cases hsUv : w.first ∈ V
       · right
         exact hsUv
       · left
-        use w.start, hs
+        use w.first, hs
         refine Connected.refl ⟨?_, hsUv⟩
-        exact Set.diff_subset <| hwVd.mem_of_mem_vx (Walk.start_vx_mem)
-    have hwfinish : w.finish ∈ h.rightSet ∪ V := Set.mem_union_right h.rightSet hv
-    have hw' : ∃ x ∈ w.vx, x ∈ V := h.crossingWalk_intersect hwVdG hwstart hwfinish
-    have := h.crossingWalk_endIf_validOn hwVdG hwstart hwfinish
+        exact Set.diff_subset <| hwVd.vx_mem_of_mem Walk.first_mem
+    have hwlast : w.last ∈ h.rightSet ∪ V := Set.mem_union_right h.rightSet hv
+    have hw' : ∃ x ∈ w.vx, x ∈ V := h.crossingWalk_intersect hwVdG hwfirst hwlast
+    have := h.crossingWalk_endIf_validOn hwVdG hwfirst hwlast
     let w' := w.endIf (P := (· ∈ V)) hw'
-    apply hUsep w'.start (by rwa [Walk.endIf_start]) w'.finish (Walk.endIf_finish hw')
+    apply hUsep w'.first (by rwa [Walk.endIf_first]) w'.last (Walk.endIf_last hw')
     rw [← vxDel_notation, induce_induce_eq_induce_right _ _ (Set.inter_subset_right.trans ?_), induce_V]
-    apply w'.connected_of_validOn
-    apply (Walk.endIf_validOn hw' hwVdG).induce
+    apply ValidIn.connected
+    apply (Walk.endIf_validIn hw' hwVdG).induce
     rintro x hx
-    exact ⟨this.mem_of_mem_vx hx, (hwVd.mem_of_mem_vx (Walk.endIf_vx_sublist hw' hx)).2⟩
+    exact ⟨this.vx_mem_of_mem hx, (hwVd.vx_mem_of_mem (Walk.endIf_vx_sublist hw' hx)).2⟩
     · exact Set.diff_subset
   · rintro hUsep
     refine hUsep.le <| induce_le _ <| Set.union_subset ?_ hV
@@ -433,47 +432,47 @@ lemma conn_sep_iff_conn_left (hVsep : G.IsVxSetSeparator V S T) (hu : u ∈ hVse
   · rintro ⟨v, hv, hconn⟩
     rw [Connected.iff_walk] at hconn
     obtain ⟨w, hwVd, rfl, rfl⟩ := hconn
-    have hw' : ∃ u ∈ w.vx, (fun x ↦ x ∈ V) u := by use w.finish, finish_vx_mem
+    have hw' : ∃ u ∈ w, (fun x ↦ x ∈ V) u := by use w.last, last_mem
     let w' := w.endIf (P := (· ∈ V)) hw'
-    use w'.finish, Walk.endIf_finish hw'
+    use w'.last, endIf_last hw'
     rw [Connected.iff_walk]
-    use w', ?_, endIf_start hw'
-    have hw'VdG : w'.ValidOn G := endIf_validOn hw' hwVd
+    use w', ?_, endIf_first hw'
+    have hw'VdG : w'.ValidIn G := endIf_validIn hw' hwVd
     refine hw'VdG.induce ?_
     rintro x hxw'
     by_cases hNonempty : w'.Nonempty
-    · by_cases hxw'Finish : x = w'.finish
+    · by_cases hxw'Last : x = w'.last
       · subst x
         right
-        exact endIf_finish hw'
-      · have hw'dVdG : w'.dropLast.ValidOn G := dropLast_validOn hw'VdG
-        have hw'dvdGV : w'.dropLast.ValidOn (G - V) := by
-          refine ValidOn.induce hw'dVdG ?_
+        exact endIf_last hw'
+      · have hw'dVdG : w'.dropLast.ValidIn G := dropLast_validIn hw'VdG
+        have hw'dvdGV : w'.dropLast.ValidIn (G - V) := by
+          refine ValidIn.induce hw'dVdG ?_
           rintro z hz
-          exact ⟨hw'dVdG.mem_of_mem_vx hz, endIf_dropLast_mem_vx hw' hNonempty hz⟩
-        have : w'.dropLast.ValidOn (G[hVsep.leftSet]) := by
-          refine ValidOn.induce hw'dVdG ?_
+          exact ⟨hw'dVdG.vx_mem_of_mem hz, endIf_dropLast_mem_vx hw' hNonempty hz⟩
+        have : w'.dropLast.ValidIn (G[hVsep.leftSet]) := by
+          refine ValidIn.induce hw'dVdG ?_
           rintro y hy
           simp only [leftSet, mem_setOf_eq]
           obtain ⟨s, hs, hsconn⟩ := hu
           use s, hs
-          rw [← endIf_start hw', ← dropLast_start hNonempty] at hsconn
+          rw [← endIf_first hw', ← dropLast_first hNonempty] at hsconn
           refine Connected.trans ?_ hsconn
-          exact w'.dropLast.connected_of_validOn_of_mem hw'dvdGV hy start_vx_mem
+          exact ValidIn.connected_of_mem hw'dvdGV hy first_mem
 
-        rw [← List.dropLast_concat_getLast vx_ne_nil, List.mem_append, ← dropLast_vx hNonempty,
-        List.mem_singleton, ← w'.finish_eq_vx_getLast] at hxw'
-        simp only [hxw'Finish, or_false] at hxw'
+        rw [mem_vxSet_iff, ← mem_notation, ← List.dropLast_concat_getLast vx_ne_nil,
+        List.mem_append, ← dropLast_vx hNonempty, List.mem_singleton, ← w'.last_eq_vx_getLast] at hxw'
+        simp only [hxw'Last, or_false] at hxw'
         left
-        exact this.mem_of_mem_vx hxw'
+        exact this.vx_mem_of_mem hxw'
     · simp only [Nonempty.not_iff] at hNonempty
       obtain ⟨y, hy⟩ := hNonempty
-      simp only [hy, nil_vx, mem_cons, not_mem_nil, or_false] at hxw'
+      simp only [hy, nil_vxSet, mem_singleton_iff] at hxw'
       subst y
       right
-      have : w'.finish = x := by
-        simp only [hy, nil_finish]
-      exact this ▸ endIf_finish hw'
+      have : w'.last = x := by
+        simp only [hy, nil_last]
+      exact this ▸ endIf_last hw'
   · rintro ⟨v, hv, hconn⟩
     use v, hv
     refine hconn.le (induce_le G ?_)
