Kura/Walk/Defs.lean
@@ -1,0 +1,629 @@
+import Kura.Operation.Subgraph
+import Kura.Operation.Minor
+import Mathlib.Data.Finset.Lattice.Basic
+import Kura.Dep.List
+import Mathlib.Data.Nat.PartENat
+
+open Set Function List Nat
+variable {α β : Type*} {G H : Graph α β} {u v x y z : α} {e e' f g : β} {S T U: Set α}
+  {F F' : Set β}
+namespace Graph
+
+
+inductive Walk (α β : Type*) where
+| nil (u : α) : Walk α β
+| cons (u : α) (e : β) (W : Walk α β) : Walk α β
+
+variable {w w₁ w₂ : Walk α β}
+namespace Walk
+
+def Nonempty : Walk α β → Prop
+| nil _ => False
+| cons _ _ _ => True
+
+def first : Walk α β → α
+| nil x => x
+| cons x _ _ => x
+
+def last : Walk α β → α
+| nil x => x
+| cons _ _ w => w.last
+
+def vx : Walk α β → List α
+| nil x => [x]
+| cons x _e w => x :: w.vx
+
+instance : Membership α (Walk α β) where
+  mem w x := x ∈ w.vx
+
+instance [DecidableEq α] : Decidable (x ∈ w) := by
+  change Decidable (x ∈ w.vx)
+  infer_instance
+
+@[simp]
+lemma mem_notation : (x ∈ w.vx) = (x ∈ w) := rfl
+
+def vxSet : Walk α β → Set α := fun w => {x | x ∈ w}
+
+def edge : Walk α β → List β
+| nil _ => []
+| cons _ e w => e :: w.edge
+
+def edgeSet : Walk α β → Set β := fun w => {e | e ∈ w.edge}
+
+def length : Walk α β → ℕ
+| nil _ => 0
+| cons _ _ w => w.length + 1
+
+def ValidIn (w : Walk α β) (G : Graph α β) : Prop :=
+  match w with
+  | nil x => x ∈ G.V
+  | cons x e w => G.Inc₂ e x w.first ∧ w.ValidIn G
+
+end Walk
+
+@[mk_iff]
+structure IsTrail (G : Graph α β) (W : Walk α β) : Prop where
+  validIn : W.ValidIn G
+  edge_nodup : W.edge.Nodup
+
+@[simp] lemma IsTrail.validIn_simp (h : G.IsTrail w) : w.ValidIn G := h.validIn
+@[simp] lemma IsTrail.edge_nodup_simp (h : G.IsTrail w) : w.edge.Nodup := h.edge_nodup
+@[simp] lemma isTrail_simp (hVd : w.ValidIn G) (hed : w.edge.Nodup) :
+    G.IsTrail w := IsTrail.mk hVd hed
+
+@[mk_iff]
+structure IsPath (G : Graph α β) (W : Walk α β) : Prop where
+  validIn : W.ValidIn G
+  nodup : W.vx.Nodup
+
+@[simp] lemma IsPath.validIn_simp (h : G.IsPath w) : w.ValidIn G := h.validIn
+@[simp] lemma IsPath.nodup_simp (h : G.IsPath w) : w.vx.Nodup := h.nodup
+@[simp] lemma isPath_simp (hVd : w.ValidIn G) (hnodup : w.vx.Nodup) :
+    G.IsPath w := IsPath.mk hVd hnodup
+
+@[mk_iff]
+structure IsWalkFrom (G : Graph α β) (S T : Set α) (W : Walk α β) : Prop where
+  validIn : W.ValidIn G
+  first_mem : W.first ∈ S
+  last_mem : W.last ∈ T
+
+@[simp] lemma IsWalkFrom.validIn_simp (h : G.IsWalkFrom S T w) : w.ValidIn G := h.validIn
+@[simp] lemma IsWalkFrom.first_mem_simp (h : G.IsWalkFrom S T w) : w.first ∈ S := h.first_mem
+@[simp] lemma IsWalkFrom.last_mem_simp (h : G.IsWalkFrom S T w) : w.last ∈ T := h.last_mem
+@[simp] lemma isWalkFrom_simp (hVd : w.ValidIn G) (hfirst : w.first ∈ S) (hlast : w.last ∈ T) :
+    G.IsWalkFrom S T w := IsWalkFrom.mk hVd hfirst hlast
+
+@[mk_iff]
+structure IsTrailFrom (G : Graph α β) (S T : Set α) (W : Walk α β) : Prop where
+  validIn : W.ValidIn G
+  edge_nodup : W.edge.Nodup
+  first_mem : W.first ∈ S
+  last_mem : W.last ∈ T
+
+@[simp] lemma IsTrailFrom.validIn_simp (h : G.IsTrailFrom S T w) : w.ValidIn G := h.validIn
+@[simp] lemma IsTrailFrom.edge_nodup_simp (h : G.IsTrailFrom S T w) : w.edge.Nodup := h.edge_nodup
+@[simp] lemma IsTrailFrom.first_mem_simp (h : G.IsTrailFrom S T w) : w.first ∈ S := h.first_mem
+@[simp] lemma IsTrailFrom.last_mem_simp (h : G.IsTrailFrom S T w) : w.last ∈ T := h.last_mem
+@[simp] lemma isTrailFrom_simp (hVd : w.ValidIn G) (hed : w.edge.Nodup) (hfirst : w.first ∈ S)
+    (hlast : w.last ∈ T) : G.IsTrailFrom S T w := IsTrailFrom.mk hVd hed hfirst hlast
+
+@[mk_iff]
+structure IsPathFrom (G : Graph α β) (S T : Set α) (W : Walk α β) : Prop where
+  validIn : W.ValidIn G
+  nodup : W.vx.Nodup
+  first_mem : W.first ∈ S
+  last_mem : W.last ∈ T
+
+@[simp] lemma IsPathFrom.validIn_simp (h : G.IsPathFrom S T w) : w.ValidIn G := h.validIn
+@[simp] lemma IsPathFrom.nodup_simp (h : G.IsPathFrom S T w) : w.vx.Nodup := h.nodup
+@[simp] lemma IsPathFrom.first_mem_simp (h : G.IsPathFrom S T w) : w.first ∈ S := h.first_mem
+@[simp] lemma IsPathFrom.last_mem_simp (h : G.IsPathFrom S T w) : w.last ∈ T := h.last_mem
+@[simp] lemma isPathFrom_simp (hVd : w.ValidIn G) (hnodup : w.vx.Nodup) (hfirst : w.first ∈ S)
+    (hlast : w.last ∈ T) : G.IsPathFrom S T w := IsPathFrom.mk hVd hnodup hfirst hlast
+
+-- def IsClosed (W : Walk α β) : Prop := W.first = W.last
+
+@[mk_iff]
+structure IsCycle (G : Graph α β) (W : Walk α β) : Prop where
+  validIn : W.ValidIn G
+  nodup' : W.vx.dropLast.Nodup
+  closed : W.first = W.last
+
+@[simp] lemma isCycle_simp (hVd : w.ValidIn G) (hnodup : w.vx.dropLast.Nodup)
+    (hclosed : w.first = w.last) : G.IsCycle w := IsCycle.mk hVd hnodup hclosed
+
+
+/- Properties between IsWalkFrom, IsTrail, IsPath, IsTrailFrom, IsPathFrom -/
+
+lemma IsTrailFrom.isTrail (h : G.IsTrailFrom S T w) : G.IsTrail w where
+  validIn := h.validIn
+  edge_nodup := h.edge_nodup
+
+lemma IsTrailFrom.isWalkFrom (h : G.IsTrailFrom S T w) : G.IsWalkFrom S T w where
+  validIn := h.validIn
+  first_mem := h.first_mem
+  last_mem := h.last_mem
+
+lemma IsPathFrom.isPath (h : G.IsPathFrom S T w) : G.IsPath w where
+  validIn := h.validIn
+  nodup := h.nodup
+
+lemma IsPathFrom.isWalkFrom (h : G.IsPathFrom S T w) : G.IsWalkFrom S T w where
+  validIn := h.validIn
+  first_mem := h.first_mem
+  last_mem := h.last_mem
+
+lemma IsPathFrom.isTrailFrom (h : G.IsPathFrom S T w) : G.IsTrailFrom S T w where
+  validIn := h.validIn
+  edge_nodup := by sorry
+  first_mem := h.first_mem
+  last_mem := h.last_mem
+
+lemma IsCycle.isTrail (h : G.IsCycle w) : G.IsTrail w where
+  validIn := h.validIn
+  edge_nodup := sorry
+
+namespace Walk
+
+/- Properties of nil -/
+
+@[simp] lemma nil_not_nonempty : ¬ (nil x : Walk α β).Nonempty := by simp [Nonempty]
+
+@[simp] lemma nil_first : (nil x : Walk α β).first = x := rfl
+
+@[simp] lemma nil_last : (nil x : Walk α β).last = x := rfl
+
+@[simp] lemma nil_vx : (nil x : Walk α β).vx = [x] := rfl
+
+@[simp] lemma mem_nil_iff : x ∈ (nil u : Walk α β) ↔ x = u := by simp [← mem_notation]
+
+@[simp] lemma nil_vxSet : (nil x : Walk α β).vxSet = {x} := by simp [vxSet]
+
+@[simp] lemma nil_edge : (nil x : Walk α β).edge = [] := rfl
+
+@[simp] lemma nil_edgeSet : (nil x : Walk α β).edgeSet = ∅ := by simp [edgeSet]
+
+@[simp] lemma nil_length : (nil x : Walk α β).length = 0 := rfl
+
+@[simp] lemma nil_injective : Injective (nil : α → Walk α β) := by
+  rintro x y h
+  rwa [nil.injEq] at h
+
+-- @[simp] lemma nil_inj : (nil x : Walk α β) = nil y ↔ x = y := by
+--   rw [nil.injEq]
+
+@[simp] lemma nil_validIn : (nil x : Walk α β).ValidIn G ↔ x ∈ G.V := by
+  simp only [ValidIn]
+
+@[simp] lemma nil_isWalkFrom : G.IsWalkFrom S T (nil x) ↔ x ∈ G.V ∧ x ∈ S ∧ x ∈ T := by
+  refine ⟨fun ⟨h, hS, hT⟩ ↦ ?_, fun ⟨hV, hS, hT⟩ ↦ ⟨?_, ?_, ?_⟩⟩ <;> simp_all only [and_self,
+  nil_validIn, nil_first, nil_last]
+
+@[simp] lemma nil_isTrail : G.IsTrail (nil x) ↔ x ∈ G.V := by
+  refine ⟨fun ⟨H1, H2⟩ ↦ ?_, fun h ↦ ⟨?_, ?_⟩⟩ <;> simp_all only [nil_validIn,
+    nil_edge, nodup_nil]
+
+@[simp] lemma nil_isPath : G.IsPath (nil x) ↔ x ∈ G.V := by
+  refine ⟨fun ⟨H1, H2⟩ ↦ ?_, fun h ↦ ⟨?_, ?_⟩⟩ <;> simp_all only [nil_vx,
+    nodup_cons, not_mem_nil, not_false_eq_true, nodup_nil, and_self, nil_validIn]
+
+@[simp] lemma nil_isTrailFrom : G.IsTrailFrom S T (nil x) ↔ x ∈ G.V ∧ x ∈ S ∧ x ∈ T := by
+  refine ⟨fun ⟨H1, H2, H3, H4⟩ ↦ ?_, fun h ↦ ⟨?_, ?_, ?_, ?_⟩⟩ <;> simp_all only [nil_validIn,
+    nil_edge, nodup_nil, nil_first, nil_last, and_self]
+
+@[simp] lemma nil_isPathFrom : G.IsPathFrom S T (nil x) ↔ x ∈ G.V ∧ x ∈ S ∧ x ∈ T := by
+  refine ⟨fun ⟨H1, H2, H3, H4⟩ ↦ ?_, fun ⟨H1, H2, H3⟩ ↦ ⟨?_, ?_, ?_, ?_⟩⟩ <;> simp_all only [nil_validIn,
+    nil_vx, nodup_cons, not_mem_nil, not_false_eq_true, nodup_nil, and_self, nil_first, nil_last]
+
+/- Properties of cons -/
+
+@[simp] lemma cons_nonempty : (cons x e w).Nonempty := by simp [Nonempty]
+
+@[simp] lemma cons_first : (cons x e w).first = x := rfl
+
+@[simp] lemma cons_last : (cons x e w).last = w.last := rfl
+
+@[simp] lemma cons_vx : (cons x e w).vx = x :: w.vx := rfl
+
+@[simp] lemma mem_cons_iff : x ∈ (cons u e w) ↔ x = u ∨ x ∈ w := by simp [← mem_notation]
+
+@[simp] lemma cons_vxSet : (cons x e w).vxSet = {x} ∪ w.vxSet := by
+  simp only [vxSet, mem_cons_iff, singleton_union]
+  rfl
+
+@[simp↓] lemma cons_vxSet_subset : (cons x e w).vxSet ⊆ U ↔ x ∈ U ∧ w.vxSet ⊆ U := by
+  simp [insert_subset_iff]
+
+@[simp] lemma cons_edge : (cons x e w).edge = e :: w.edge := rfl
+
+@[simp] lemma cons_edgeSet : (cons x e w).edgeSet = {e} ∪ w.edgeSet := by
+  simp only [edgeSet, cons_edge, mem_cons, singleton_union]
+  rfl
+
+@[simp] lemma cons_length : (cons x e w).length = w.length + 1 := rfl
+
+@[simp] lemma cons_validIn : (cons x e w).ValidIn G ↔ G.Inc₂ e x w.first ∧ w.ValidIn G :=
+  ⟨id, id⟩
+
+@[simp]
+lemma ValidIn.cons (hw : (cons x e w).ValidIn G) : w.ValidIn G := by
+  rw [cons_validIn] at hw
+  exact hw.2
+
+@[simp] lemma cons_isWalkFrom : G.IsWalkFrom S T (cons x e w) ↔
+    w.ValidIn G ∧ G.Inc₂ e x w.first ∧ x ∈ S ∧ w.last ∈ T := by
+  refine ⟨fun ⟨h, hS, hT⟩ ↦ ⟨?_, ?_, ?_, ?_⟩, fun ⟨hV, hS, hVd, hT⟩ ↦ ⟨?_, ?_, ?_⟩⟩
+  <;> simp_all only [cons_validIn, cons_first, cons_last, and_self]
+
+@[simp]
+lemma cons_vx_nodup (h : (cons x e w).vx.Nodup) : w.vx.Nodup := by
+  simp only [cons_vx, nodup_cons] at h
+  exact h.2
+
+@[simp] lemma cons_isTrail : G.IsTrail (cons x e w) ↔
+    G.IsTrail w ∧ G.Inc₂ e x w.first ∧ e ∉ w.edge := by
+  refine ⟨fun ⟨H1, H2⟩ ↦ ⟨⟨?_, ?_⟩, ?_, ?_⟩, fun ⟨hT, h₂, hnin⟩ ↦ ⟨?_, ?_⟩⟩
+  · rw [cons_validIn] at H1
+    exact H1.2
+  · simp only [cons_edge, nodup_cons] at H2
+    exact H2.2
+  · rw [cons_validIn] at H1
+    exact H1.1
+  · simp only [cons_edge, nodup_cons] at H2
+    exact H2.1
+  · simp [h₂, hT]
+  · simp [hT.edge_nodup, hnin]
+
+@[simp]
+lemma IsTrail.cons (h : G.IsTrail (cons x e w)) : G.IsTrail w := by
+  rw [cons_isTrail] at h
+  exact h.1
+
+@[simp] lemma cons_isPath : G.IsPath (cons x e w) ↔ G.IsPath w ∧ G.Inc₂ e x w.first ∧ x ∉ w := by
+  constructor
+  · refine fun ⟨hVd, hnodup⟩ ↦ ⟨?_, ?_, ?_⟩ <;> simp_all only [cons_validIn, cons_vx,
+    nodup_cons, mem_notation, not_false_eq_true, isPath_simp]
+  · refine fun ⟨hP, h₂, hnin⟩ ↦ ⟨?_, ?_⟩ <;> simp_all only [not_false_eq_true,
+    and_self, cons_vx, nodup_cons, mem_notation, true_and, hP.validIn, hP.nodup, cons_validIn]
+
+@[simp]
+lemma IsPath.cons (h : G.IsPath (cons x e w)) : G.IsPath w := by
+  rw [cons_isPath] at h
+  exact h.1
+
+@[simp]
+lemma cons_isTrailFrom : G.IsTrailFrom S T (cons x e w) ↔
+    G.IsTrail w ∧ G.Inc₂ e x w.first ∧ e ∉ w.edge ∧ x ∈ S ∧ w.last ∈ T := by
+  constructor
+  · refine fun ⟨hVd, hnodup, hfirst, hlast⟩ ↦ ⟨?_, ?_, ?_, ?_, ?_⟩ <;> simp_all only [cons_validIn,
+    cons_edge, nodup_cons, cons_first, cons_last, isTrail_simp, not_false_eq_true]
+  · refine fun ⟨hV, hS, hVd, hT⟩ ↦ ⟨?_, ?_, ?_, ?_⟩ <;> simp_all only [IsTrail.validIn_simp,
+    not_false_eq_true, and_self, cons_edge, nodup_cons, true_and, cons_isTrail, cons_first,
+    cons_last, hV.edge_nodup]
+
+@[simp]
+lemma cons_isPathFrom : G.IsPathFrom S T (cons x e w) ↔
+    G.IsPath w ∧ G.Inc₂ e x w.first ∧ x ∉ w ∧ x ∈ S ∧ w.last ∈ T := by
+  refine ⟨fun ⟨hVd, hnodup, hfirst, hlast⟩ ↦ ⟨?_, ?_, ?_, ?_, ?_⟩, fun ⟨hV, hS, hVd, hT⟩ ↦ ⟨?_, ?_, ?_, ?_⟩⟩
+  <;> simp_all only [not_false_eq_true, and_self, cons_edge, nodup_cons, cons_validIn, cons_first,
+  cons_last, mem_notation, cons_vx, isPath_simp, cons_isPath, true_and, IsPath.validIn]
+  exact hV.nodup
+
+/- Properties between the basic properties of a walk -/
+
+lemma vx_ne_nil : w.vx ≠ [] := by
+  match w with
+  | nil x => simp
+  | cons x e w => simp
+
+@[simp] lemma mem_vxSet_iff : x ∈ w.vxSet ↔ x ∈ w := by simp [vxSet]
+
+@[simp] lemma mem_edgeSet_iff : e ∈ w.edgeSet ↔ e ∈ w.edge := by simp [edgeSet]
+
+@[simp] lemma first_mem : w.first ∈ w := by
+  match w with
+  | nil x => simp
+  | cons x e w => simp
+
+@[simp] lemma first_mem_vxSet : w.first ∈ w.vxSet := by simp
+
+lemma first_eq_vx_head : w.first = w.vx.head vx_ne_nil := by
+  match w with
+  | nil x => rfl
+  | cons x e w => rfl
+
+@[simp]
+lemma last_mem {w : Walk α β} : w.last ∈ w := by
+  match w with
+  | nil x => simp
+  | cons x e w => simp [last_mem]
+
+@[simp]
+lemma last_mem_vxSet : w.last ∈ w.vxSet := by simp
+
+lemma last_eq_vx_getLast {w : Walk α β} : w.last = w.vx.getLast vx_ne_nil := by
+  match w with
+  | nil x => rfl
+  | cons x e w =>
+    simp only [cons_last, cons_vx, ne_eq, vx_ne_nil, not_false_eq_true, getLast_cons]
+    apply last_eq_vx_getLast
+
+lemma ValidIn.vx_mem_of_mem {w : Walk α β} (h : w.ValidIn G) (hmem : x ∈ w) : x ∈ G.V := by
+  match w with
+  | .nil y =>
+    rw [mem_nil_iff] at hmem
+    exact mem_of_eq_of_mem hmem h
+  | .cons y e w =>
+    obtain ⟨hbtw, hVd⟩ := h
+    obtain rfl | h : x = y ∨ x ∈ w := by simpa using hmem
+    · exact hbtw.vx_mem_left
+    · exact hVd.vx_mem_of_mem h
+
+lemma ValidIn.vxSet_subset (hVd : w.ValidIn G) : w.vxSet ⊆ G.V := fun _ ↦ hVd.vx_mem_of_mem
+
+lemma ValidIn.edge_mem_of_mem {w : Walk α β} (h : w.ValidIn G) (hmem : e ∈ w.edge) : e ∈ G.E := by
+  match w with
+  | .nil x => simp at hmem
+  | .cons x e' w =>
+    obtain ⟨hbtw, hVd⟩ := h
+    obtain rfl | h : e = e' ∨ e ∈ w.edge := by simpa using hmem
+    · exact hbtw.edge_mem
+    · exact hVd.edge_mem_of_mem h
+
+lemma ValidIn.edgeSet_subset (h : w.ValidIn G) : w.edgeSet ⊆ G.E := fun _ ↦ h.edge_mem_of_mem
+
+/- Properties of Nonempty -/
+
+lemma Nonempty.exists_cons : w.Nonempty → ∃ x e w', w = cons x e w' := by
+  induction w with
+  | nil x => simp only [Nonempty, reduceCtorEq, exists_false, imp_self]
+  | cons x e w ih => simp only [cons.injEq, exists_and_left, exists_eq', and_true, implies_true]
+
+lemma Nonempty.iff_exists_cons : w.Nonempty ↔ ∃ x e w', w = cons x e w' := by
+  constructor
+  · apply Nonempty.exists_cons
+  · rintro ⟨x, e, w', rfl⟩
+    simp [Nonempty, cons.injEq]
+
+@[simp]
+lemma Nonempty.not_nil : ¬ (nil x : Walk α β).Nonempty := by
+  simp only [Nonempty, not_false_eq_true]
+
+@[simp]
+lemma Nonempty.cons_true : (cons x e w).Nonempty := by
+  simp only [Nonempty]
+
+@[simp]
+lemma Nonempty.not_iff : ¬ w.Nonempty ↔ ∃ x, w = nil x := by
+  match w with
+  | nil x => simp only [not_nil, not_false_eq_true, nil.injEq, exists_eq']
+  | cons x e w => simp only [Nonempty, not_true_eq_false, reduceCtorEq, exists_false]
+
+@[simp]
+lemma Nonempty.iff_length_pos : 0 < w.length ↔ w.Nonempty := by
+  constructor
+  · rintro hlen
+    by_contra! h
+    simp only [not_iff] at h
+    obtain ⟨x, rfl⟩ := h
+    simp at hlen
+  · rw [Nonempty.iff_exists_cons]
+    rintro ⟨x, e, w, rfl⟩
+    simp only [cons_length, lt_add_iff_pos_left, add_pos_iff, lt_one_iff, pos_of_gt, or_true]
+
+lemma first_eq_last_of_not_nonempty (h : ¬ w.Nonempty) : w.first = w.last := by
+  match w with
+  | nil x => simp only [nil_first, nil_last]
+  | cons x e w => simp only [Nonempty.cons_true, not_true_eq_false] at h
+
+@[simp]
+lemma first_eq_last_iff (hnodup : w.vx.Nodup) : w.first = w.last ↔ ¬ w.Nonempty := by
+  match w with
+  | .nil x => simp only [nil_first, nil_last, Nonempty.not_nil, not_false_eq_true]
+  | .cons x e w =>
+    simp only [cons_vx, nodup_cons, cons_first, cons_last, Nonempty.cons_true, not_true_eq_false,
+      iff_false, ne_eq] at hnodup ⊢
+    exact fun h => hnodup.1 (h ▸ last_mem)
+
+@[simp]
+lemma first_ne_last_iff (hnodup : w.vx.Nodup) : w.first ≠ w.last ↔ w.Nonempty :=
+  (first_eq_last_iff hnodup).not_left
+
+end Walk
+open Walk
+
+def Inc₂.walk (_h : G.Inc₂ e u v) : Walk α β := cons u e (nil v)
+
+namespace Inc₂
+
+@[simp] lemma walk_first (h : G.Inc₂ e u v): h.walk.first = u := rfl
+
+@[simp] lemma walk_last (h : G.Inc₂ e u v): h.walk.last = v := rfl
+
+@[simp] lemma walk_vx (h : G.Inc₂ e u v): h.walk.vx = [u, v] := rfl
+
+@[simp] lemma mem_walk_iff (h : G.Inc₂ e u v) (x : α) : x ∈ h.walk ↔ x = u ∨ x = v := by
+  simp [walk]
+
+@[simp] lemma walk_vxSet (h : G.Inc₂ e u v): h.walk.vxSet = {u, v} := by
+  simp only [vxSet, mem_walk_iff]
+  rfl
+
+@[simp] lemma walk_edge (h : G.Inc₂ e u v): h.walk.edge = [e] := rfl
+
+@[simp] lemma walk_edgeSet (h : G.Inc₂ e u v): h.walk.edgeSet = {e} := by simp [edgeSet]
+
+@[simp] lemma walk_length (h : G.Inc₂ e u v): h.walk.length = 1 := rfl
+
+lemma walk_validIn (h : G.Inc₂ e u v) : h.walk.ValidIn G := by
+  simp [walk, h, h.vx_mem_right]
+
+lemma walk_isPath (h : G.Inc₂ e u v) (hne : u ≠ v) : G.IsPath h.walk :=
+  ⟨h.walk_validIn, by simp [hne]⟩
+
+
+lemma mem_left_of_edge_mem_walk (h : G.Inc₂ e u v) (he : e ∈ w.edge) (hVd : w.ValidIn G) :
+    u ∈ w := by
+  induction w with
+  | nil x => simp at he
+  | cons x e' w ih =>
+    simp only [cons_edge, mem_cons, cons_vx] at he ⊢
+    obtain rfl | he' := he
+    · obtain ⟨hbtw, hVd⟩ := hVd
+      obtain ⟨rfl, rfl⟩ | ⟨rfl, rfl⟩ := hbtw.eq_or_eq_of_inc₂ h
+      · left
+      · right
+        exact first_mem
+    · right
+      exact ih he' hVd.2
+
+lemma mem_right_of_edge_mem_walk (h : G.Inc₂ e u v) (he : e ∈ w.edge) (hVd : w.ValidIn G) :
+    v ∈ w := h.symm.mem_left_of_edge_mem_walk he hVd
+
+end Inc₂
+
+/-- Given a graph adjacency, we can create a walk of length 1 -/
+lemma Adj.exist_walk (h : G.Adj u v) : ∃ (W : Walk α β), W.ValidIn G ∧ W.length = 1 ∧ W.first = u ∧
+    W.last = v := by
+  obtain ⟨e, he⟩ := h
+  use he.walk, he.walk_validIn
+  simp only [Inc₂.walk_length, Inc₂.walk_first, Inc₂.walk_last, and_self]
+
+/-- Given a reflexive adjacency, we can create a walk of length at most 1 -/
+lemma reflAdj.exist_walk (h : G.reflAdj u v) : ∃ (W : Walk α β), W.ValidIn G ∧ W.length ≤ 1 ∧
+    W.first = u ∧ W.last = v := by
+  obtain hadj | ⟨rfl, hx⟩ := h
+  · obtain ⟨W, hW, hlength, hfirst, hlast⟩ := hadj.exist_walk
+    use W, hW
+    simp only [hlength, le_refl, hfirst, hlast, and_self]
+  · use nil u
+    constructor
+    · simp [hx]
+    · simp
+
+namespace Walk
+
+lemma ValidIn.connected (h : w.ValidIn G) : G.Connected w.first w.last := by
+  induction w with
+  | nil x => simpa only [nil_first, nil_last, Connected.refl_iff]
+  | cons x e w ih =>
+    obtain ⟨H1, H2⟩ := h
+    simp only [cons_first, cons_last]
+    exact H1.connected.trans (ih H2)
+
+lemma ValidIn.connected_last_of_mem (h : w.ValidIn G) (hx : u ∈ w) : G.Connected u w.last := by
+  induction w generalizing u with
+  | nil x =>
+    rw [mem_nil_iff] at hx
+    subst u
+    simp only [nil_last, Connected.refl_iff]
+    exact h
+  | cons x e w ih =>
+    rw [mem_cons_iff] at hx
+    obtain rfl | hx := hx
+    · exact Connected.trans h.1.connected (ih h.2 (first_mem))
+    · exact ih h.2 hx
+
+lemma ValidIn.connected_of_mem (h : w.ValidIn G) (hx : x ∈ w) (hy : y ∈ w) :
+    G.Connected x y := by
+  have hx' := ValidIn.connected_last_of_mem h hx
+  have hy' := ValidIn.connected_last_of_mem h hy
+  exact Connected.trans hx' hy'.symm
+
+lemma ValidIn.connected_first_of_mem (h : w.ValidIn G) (hx : x ∈ w) : G.Connected w.first x :=
+  h.connected_of_mem first_mem hx
+
+/-- A subgraph inherits all valid walks -/
+lemma ValidIn.le {w : Walk α β} (h : w.ValidIn G) (hle : G ≤ H) : w.ValidIn H := by
+  match w with
+  | .nil x => exact vx_subset_of_le hle h
+  | .cons x e w =>
+    obtain ⟨hbtw, hVd⟩ := h
+    exact ⟨hbtw.le hle, hVd.le hle⟩
+
+lemma IsWalkFrom.le (h : G.IsWalkFrom S T w) (hle : G ≤ H) : H.IsWalkFrom S T w where
+  validIn := h.validIn.le hle
+  first_mem := h.first_mem
+  last_mem := h.last_mem
+
+lemma IsPath.le (hp : G.IsPath w) (hle : G ≤ H) : H.IsPath w where
+  validIn := hp.validIn.le hle
+  nodup := hp.nodup
+
+lemma IsPathFrom.le (hp : G.IsPathFrom S T w) (hle : G ≤ H) : H.IsPathFrom S T w where
+  validIn := hp.validIn.le hle
+  nodup := hp.nodup
+  first_mem := hp.first_mem
+  last_mem := hp.last_mem
+
+lemma ValidIn.eq_nil_of_mem_isolated {w : Walk α β} {x : α} (hisol : G.Isolated x) (hmem : x ∈ w)
+    (h : w.ValidIn G) : w = nil x := by
+  match w with
+  | .nil y => simp_all only [mem_nil_iff, nil_validIn]
+  | .cons y e w =>
+    exfalso
+    obtain ⟨hbtw, hVd⟩ := h
+    rw [mem_cons_iff] at hmem
+    obtain rfl | h := hmem
+    · exact hisol e hbtw.inc_left
+    · have := ValidIn.eq_nil_of_mem_isolated hisol h hVd
+      subst w
+      rw [nil_first] at hbtw
+      exact hisol e hbtw.inc_right
+
+lemma ValidIn.induce (hVd : w.ValidIn G) (hU : w.vxSet ⊆ U) : w.ValidIn (G[U]) := by
+  induction w with
+  | nil x => simpa using hU
+  | cons x e w ih =>
+    obtain ⟨hbtw, hVd⟩ := hVd
+    obtain ⟨hUx, hUw⟩ := by simpa [cons_vxSet_subset] using hU
+    refine ⟨?_, ih hVd hUw⟩
+    simp only [induce_inc₂_iff, hbtw, hUx, true_and]
+    exact hUw first_mem_vxSet
+
+-- Not true : Take a trivial walk on some vertex v ∈ U \ G.V
+-- lemma ValidIn.induce_iff : w.ValidIn (G[U]) ↔ w.ValidIn G ∧ ∀ x ∈ w, x ∈ U := by
+
+lemma ValidIn.vxDel (hVd : w.ValidIn G) (hU : Disjoint w.vxSet U) : w.ValidIn (G - U) :=
+  ValidIn.induce hVd (subset_diff.mpr ⟨hVd.vxSet_subset, hU⟩)
+
+@[simp]
+lemma validIn_vxDel_iff : w.ValidIn (G - U) ↔ w.ValidIn G ∧ Disjoint w.vxSet U := by
+  constructor
+  · rintro h
+    refine ⟨h.le (vxDel_le G), ?_⟩
+    rintro V hVw hVU x hxV
+    exact (h.vxSet_subset <| hVw hxV).2 <| hVU hxV
+  · rintro ⟨hVd, hU⟩
+    exact ValidIn.vxDel hVd hU
+
+lemma ValidIn.restrict (hVd : w.ValidIn G) (hF : w.edgeSet ⊆ F) : w.ValidIn (G{F}) := by
+  induction w with
+  | nil x => exact hVd
+  | cons x e w ih =>
+    obtain ⟨hbtw, hVd⟩ := hVd
+    specialize ih hVd (fun e' he' => hF (by simp [he']))
+    simp only [cons_validIn, restrict_inc₂, hbtw, true_and, ih, and_true]
+    exact hF (by simp [cons_edge])
+
+@[simp]
+lemma validIn_restrict_iff : w.ValidIn (G{F}) ↔ w.ValidIn G ∧ w.edgeSet ⊆ F := by
+  constructor
+  · rintro h
+    refine ⟨h.le (restrict_le G F), ?_⟩
+    rintro e he
+    exact (h.edgeSet_subset he).2
+  · rintro ⟨hVd, hF⟩
+    exact ValidIn.restrict hVd hF
+
+@[simp]
+lemma validIn_edgeDel_iff : w.ValidIn (G \ F) ↔ w.ValidIn G ∧ Disjoint w.edgeSet F := by
+  rw [edgeDel, validIn_restrict_iff, and_congr_right_iff]
+  rintro hVd
+  simp only [subset_diff, hVd.edgeSet_subset, true_and]
+
+lemma ValidIn.subgraph (hVd : w.ValidIn G) (hU : w.vxSet ⊆ U) (hF : w.edgeSet ⊆ F) :
+    w.ValidIn (G{F}[U]) := ValidIn.induce (ValidIn.restrict hVd hF) hU
+
+end Walk
